Port BT2D to Array2

dist/Klas_GEMM_BlockTiling2D.cu
@@ -35,6 +35,7 @@ __hoisted_0(float alpha,
             for (; k < 4U; k++)
                 sA[(col + k) * 32U + row] = local[k];
         }
+        uint32_t __anf06 = bkIdx;
         float *tileB = gB;
         uint32_t i = 0U;
         for (; i < 1024U; i += 64U) {
@@ -43,7 +44,7 @@ __hoisted_0(float alpha,
             uint32_t row = (i + threadIdx.x * 4U) / 32U;
             uint32_t col = (i + threadIdx.x * 4U) % 32U;
             vec_memcpy(local,
-                       tileB + cols * (__anf03 * 32U) + mcol * 32U +
+                       tileB + cols * (__anf06 * 32U) + mcol * 32U +
                        cols * row + col);
             uint32_t k = 0U;
             for (; k < 4U; k++)
@@ -77,14 +78,15 @@ __hoisted_0(float alpha,
     for (; resIdxM < 8U; resIdxM++) {
         uint32_t resIdxN = 0U;
         for (; resIdxN < 8U; resIdxN++)
-            t_tile[(blockIdx.x / (cols / 32U) * 32U + threadIdx.x / 4U * 8U +
-                    resIdxM) * cols + blockIdx.x % (cols / 32U) * 32U +
-                   threadIdx.x % 4U * 8U + resIdxN]
+            t_tile[(32U * (blockIdx.x / (cols / 32U)) +
+                    8U * (threadIdx.x / 4U) + resIdxM) * cols +
+                   32U * (blockIdx.x % (cols / 32U)) + 8U * (threadIdx.x % 4U) +
+                   resIdxN]
                 = beta *
-                t_tile[(blockIdx.x / (cols / 32U) * 32U +
-                        threadIdx.x / 4U * 8U + resIdxM) * cols +
-                       blockIdx.x % (cols / 32U) * 32U + threadIdx.x % 4U * 8U +
-                       resIdxN]
+                t_tile[(32U * (blockIdx.x / (cols / 32U)) +
+                        8U * (threadIdx.x / 4U) + resIdxM) * cols +
+                       32U * (blockIdx.x % (cols / 32U)) +
+                       8U * (threadIdx.x % 4U) + resIdxN]
                 + alpha * rchProd[resIdxM * 8U + resIdxN];
     }
 }
@@ -142,6 +144,7 @@ __hoisted_1(float alpha,
             for (; k < 4U; k++)
                 sA[(col + k) * 32U + row] = local[k];
         }
+        uint32_t __anf06 = bkIdx;
         float *tileB = gB;
         uint32_t i = 0U;
         for (; i < 1024U; i += 32U) {
@@ -150,7 +153,7 @@ __hoisted_1(float alpha,
             uint32_t row = (i + threadIdx.x * 4U) / 32U;
             uint32_t col = (i + threadIdx.x * 4U) % 32U;
             vec_memcpy(local,
-                       tileB + cols * (__anf03 * 32U) + mcol * 32U +
+                       tileB + cols * (__anf06 * 32U) + mcol * 32U +
                        cols * row + col);
             uint32_t k = 0U;
             for (; k < 4U; k++)
@@ -184,14 +187,15 @@ __hoisted_1(float alpha,
     for (; resIdxM < 8U; resIdxM++) {
         uint32_t resIdxN = 0U;
         for (; resIdxN < 16U; resIdxN++)
-            t_tile[(blockIdx.x / (cols / 32U) * 32U + threadIdx.x / 2U * 8U +
-                    resIdxM) * cols + blockIdx.x % (cols / 32U) * 32U +
-                   threadIdx.x % 2U * 16U + resIdxN]
+            t_tile[(32U * (blockIdx.x / (cols / 32U)) +
+                    8U * (threadIdx.x / 2U) + resIdxM) * cols +
+                   32U * (blockIdx.x % (cols / 32U)) +
+                   16U * (threadIdx.x % 2U) + resIdxN]
                 = beta *
-                t_tile[(blockIdx.x / (cols / 32U) * 32U +
-                        threadIdx.x / 2U * 8U + resIdxM) * cols +
-                       blockIdx.x % (cols / 32U) * 32U +
-                       threadIdx.x % 2U * 16U + resIdxN]
+                t_tile[(32U * (blockIdx.x / (cols / 32U)) +
+                        8U * (threadIdx.x / 2U) + resIdxM) * cols +
+                       32U * (blockIdx.x % (cols / 32U)) +
+                       16U * (threadIdx.x % 2U) + resIdxN]
                 + alpha * rchProd[resIdxM * 16U + resIdxN];
     }
 }
@@ -250,6 +254,7 @@ __hoisted_2(float alpha,
             for (; k < 4U; k++)
                 sA[(col + k) * 32U + row] = local[k];
         }
+        uint32_t __anf06 = bkIdx;
         float *tileB = gB;
         uint32_t i = 0U;
         for (; i < 1024U; i += 32U) {
@@ -258,7 +263,7 @@ __hoisted_2(float alpha,
             uint32_t row = (i + threadIdx.x * 4U) / 32U;
             uint32_t col = (i + threadIdx.x * 4U) % 32U;
             vec_memcpy(local,
-                       tileB + cols * (__anf03 * 32U) + mcol * 32U +
+                       tileB + cols * (__anf06 * 32U) + mcol * 32U +
                        cols * row + col);
             uint32_t k = 0U;
             for (; k < 4U; k++)
@@ -292,14 +297,15 @@ __hoisted_2(float alpha,
     for (; resIdxM < 16U; resIdxM++) {
         uint32_t resIdxN = 0U;
         for (; resIdxN < 8U; resIdxN++)
-            t_tile[(blockIdx.x / (cols / 32U) * 32U + threadIdx.x / 4U * 16U +
-                    resIdxM) * cols + blockIdx.x % (cols / 32U) * 32U +
-                   threadIdx.x % 4U * 8U + resIdxN]
+            t_tile[(32U * (blockIdx.x / (cols / 32U)) +
+                    16U * (threadIdx.x / 4U) + resIdxM) * cols +
+                   32U * (blockIdx.x % (cols / 32U)) + 8U * (threadIdx.x % 4U) +
+                   resIdxN]
                 = beta *
-                t_tile[(blockIdx.x / (cols / 32U) * 32U +
-                        threadIdx.x / 4U * 16U + resIdxM) * cols +
-                       blockIdx.x % (cols / 32U) * 32U + threadIdx.x % 4U * 8U +
-                       resIdxN]
+                t_tile[(32U * (blockIdx.x / (cols / 32U)) +
+                        16U * (threadIdx.x / 4U) + resIdxM) * cols +
+                       32U * (blockIdx.x % (cols / 32U)) +
+                       8U * (threadIdx.x % 4U) + resIdxN]
                 + alpha * rchProd[resIdxM * 8U + resIdxN];
     }
 }
@@ -358,6 +364,7 @@ __hoisted_3(float alpha,
             for (; k < 4U; k++)
                 sA[(col + k) * 32U + row] = local[k];
         }
+        uint32_t __anf06 = bkIdx;
         float *tileB = gB;
         uint32_t i = 0U;
         for (; i < 1024U; i += 16U) {
@@ -366,7 +373,7 @@ __hoisted_3(float alpha,
             uint32_t row = (i + threadIdx.x * 4U) / 32U;
             uint32_t col = (i + threadIdx.x * 4U) % 32U;
             vec_memcpy(local,
-                       tileB + cols * (__anf03 * 32U) + mcol * 32U +
+                       tileB + cols * (__anf06 * 32U) + mcol * 32U +
                        cols * row + col);
             uint32_t k = 0U;
             for (; k < 4U; k++)
@@ -400,14 +407,15 @@ __hoisted_3(float alpha,
     for (; resIdxM < 16U; resIdxM++) {
         uint32_t resIdxN = 0U;
         for (; resIdxN < 16U; resIdxN++)
-            t_tile[(blockIdx.x / (cols / 32U) * 32U + threadIdx.x / 2U * 16U +
-                    resIdxM) * cols + blockIdx.x % (cols / 32U) * 32U +
-                   threadIdx.x % 2U * 16U + resIdxN]
+            t_tile[(32U * (blockIdx.x / (cols / 32U)) +
+                    16U * (threadIdx.x / 2U) + resIdxM) * cols +
+                   32U * (blockIdx.x % (cols / 32U)) +
+                   16U * (threadIdx.x % 2U) + resIdxN]
                 = beta *
-                t_tile[(blockIdx.x / (cols / 32U) * 32U +
-                        threadIdx.x / 2U * 16U + resIdxM) * cols +
-                       blockIdx.x % (cols / 32U) * 32U +
-                       threadIdx.x % 2U * 16U + resIdxN]
+                t_tile[(32U * (blockIdx.x / (cols / 32U)) +
+                        16U * (threadIdx.x / 2U) + resIdxM) * cols +
+                       32U * (blockIdx.x % (cols / 32U)) +
+                       16U * (threadIdx.x % 2U) + resIdxN]
                 + alpha * rchProd[resIdxM * 16U + resIdxN];
     }
 }
@@ -466,6 +474,7 @@ __hoisted_4(float alpha,
             for (; k < 4U; k++)
                 sA[(col + k) * 32U + row] = local[k];
         }
+        uint32_t __anf06 = bkIdx;
         float *tileB = gB;
         uint32_t i = 0U;
         for (; i < 2048U; i += 64U) {
@@ -474,7 +483,7 @@ __hoisted_4(float alpha,
             uint32_t row = (i + threadIdx.x * 4U) / 32U;
             uint32_t col = (i + threadIdx.x * 4U) % 32U;
             vec_memcpy(local,
-                       tileB + cols * (__anf03 * 64U) + mcol * 32U +
+                       tileB + cols * (__anf06 * 64U) + mcol * 32U +
                        cols * row + col);
             uint32_t k = 0U;
             for (; k < 4U; k++)
@@ -508,14 +517,15 @@ __hoisted_4(float alpha,
     for (; resIdxM < 8U; resIdxM++) {
         uint32_t resIdxN = 0U;
         for (; resIdxN < 8U; resIdxN++)
-            t_tile[(blockIdx.x / (cols / 32U) * 32U + threadIdx.x / 4U * 8U +
-                    resIdxM) * cols + blockIdx.x % (cols / 32U) * 32U +
-                   threadIdx.x % 4U * 8U + resIdxN]
+            t_tile[(32U * (blockIdx.x / (cols / 32U)) +
+                    8U * (threadIdx.x / 4U) + resIdxM) * cols +
+                   32U * (blockIdx.x % (cols / 32U)) + 8U * (threadIdx.x % 4U) +
+                   resIdxN]
                 = beta *
-                t_tile[(blockIdx.x / (cols / 32U) * 32U +
-                        threadIdx.x / 4U * 8U + resIdxM) * cols +
-                       blockIdx.x % (cols / 32U) * 32U + threadIdx.x % 4U * 8U +
-                       resIdxN]
+                t_tile[(32U * (blockIdx.x / (cols / 32U)) +
+                        8U * (threadIdx.x / 4U) + resIdxM) * cols +
+                       32U * (blockIdx.x % (cols / 32U)) +
+                       8U * (threadIdx.x % 4U) + resIdxN]
                 + alpha * rchProd[resIdxM * 8U + resIdxN];
     }
 }
@@ -573,6 +583,7 @@ __hoisted_5(float alpha,
             for (; k < 4U; k++)
                 sA[(col + k) * 32U + row] = local[k];
         }
+        uint32_t __anf06 = bkIdx;
         float *tileB = gB;
         uint32_t i = 0U;
         for (; i < 2048U; i += 32U) {
@@ -581,7 +592,7 @@ __hoisted_5(float alpha,
             uint32_t row = (i + threadIdx.x * 4U) / 32U;
             uint32_t col = (i + threadIdx.x * 4U) % 32U;
             vec_memcpy(local,
-                       tileB + cols * (__anf03 * 64U) + mcol * 32U +
+                       tileB + cols * (__anf06 * 64U) + mcol * 32U +
                        cols * row + col);
             uint32_t k = 0U;
             for (; k < 4U; k++)
@@ -615,14 +626,15 @@ __hoisted_5(float alpha,
     for (; resIdxM < 8U; resIdxM++) {
         uint32_t resIdxN = 0U;
         for (; resIdxN < 16U; resIdxN++)
-            t_tile[(blockIdx.x / (cols / 32U) * 32U + threadIdx.x / 2U * 8U +
-                    resIdxM) * cols + blockIdx.x % (cols / 32U) * 32U +
-                   threadIdx.x % 2U * 16U + resIdxN]
+            t_tile[(32U * (blockIdx.x / (cols / 32U)) +
+                    8U * (threadIdx.x / 2U) + resIdxM) * cols +
+                   32U * (blockIdx.x % (cols / 32U)) +
+                   16U * (threadIdx.x % 2U) + resIdxN]
                 = beta *
-                t_tile[(blockIdx.x / (cols / 32U) * 32U +
-                        threadIdx.x / 2U * 8U + resIdxM) * cols +
-                       blockIdx.x % (cols / 32U) * 32U +
-                       threadIdx.x % 2U * 16U + resIdxN]
+                t_tile[(32U * (blockIdx.x / (cols / 32U)) +
+                        8U * (threadIdx.x / 2U) + resIdxM) * cols +
+                       32U * (blockIdx.x % (cols / 32U)) +
+                       16U * (threadIdx.x % 2U) + resIdxN]
                 + alpha * rchProd[resIdxM * 16U + resIdxN];
     }
 }
@@ -681,6 +693,7 @@ __hoisted_6(float alpha,
             for (; k < 4U; k++)
                 sA[(col + k) * 32U + row] = local[k];
         }
+        uint32_t __anf06 = bkIdx;
         float *tileB = gB;
         uint32_t i = 0U;
         for (; i < 2048U; i += 32U) {
@@ -689,7 +702,7 @@ __hoisted_6(float alpha,
             uint32_t row = (i + threadIdx.x * 4U) / 32U;
             uint32_t col = (i + threadIdx.x * 4U) % 32U;
             vec_memcpy(local,
-                       tileB + cols * (__anf03 * 64U) + mcol * 32U +
+                       tileB + cols * (__anf06 * 64U) + mcol * 32U +
                        cols * row + col);
             uint32_t k = 0U;
             for (; k < 4U; k++)
@@ -723,14 +736,15 @@ __hoisted_6(float alpha,
     for (; resIdxM < 16U; resIdxM++) {
         uint32_t resIdxN = 0U;
         for (; resIdxN < 8U; resIdxN++)
-            t_tile[(blockIdx.x / (cols / 32U) * 32U + threadIdx.x / 4U * 16U +
-                    resIdxM) * cols + blockIdx.x % (cols / 32U) * 32U +
-                   threadIdx.x % 4U * 8U + resIdxN]
+            t_tile[(32U * (blockIdx.x / (cols / 32U)) +
+                    16U * (threadIdx.x / 4U) + resIdxM) * cols +
+                   32U * (blockIdx.x % (cols / 32U)) + 8U * (threadIdx.x % 4U) +
+                   resIdxN]
                 = beta *
-                t_tile[(blockIdx.x / (cols / 32U) * 32U +
-                        threadIdx.x / 4U * 16U + resIdxM) * cols +
-                       blockIdx.x % (cols / 32U) * 32U + threadIdx.x % 4U * 8U +
-                       resIdxN]
+                t_tile[(32U * (blockIdx.x / (cols / 32U)) +
+                        16U * (threadIdx.x / 4U) + resIdxM) * cols +
+                       32U * (blockIdx.x % (cols / 32U)) +
+                       8U * (threadIdx.x % 4U) + resIdxN]
                 + alpha * rchProd[resIdxM * 8U + resIdxN];
     }
 }
@@ -789,6 +803,7 @@ __hoisted_7(float alpha,
             for (; k < 4U; k++)
                 sA[(col + k) * 32U + row] = local[k];
         }
+        uint32_t __anf06 = bkIdx;
         float *tileB = gB;
         uint32_t i = 0U;
         for (; i < 2048U; i += 16U) {
@@ -797,7 +812,7 @@ __hoisted_7(float alpha,
             uint32_t row = (i + threadIdx.x * 4U) / 32U;
             uint32_t col = (i + threadIdx.x * 4U) % 32U;
             vec_memcpy(local,
-                       tileB + cols * (__anf03 * 64U) + mcol * 32U +
+                       tileB + cols * (__anf06 * 64U) + mcol * 32U +
                        cols * row + col);
             uint32_t k = 0U;
             for (; k < 4U; k++)
@@ -831,14 +846,15 @@ __hoisted_7(float alpha,
     for (; resIdxM < 16U; resIdxM++) {
         uint32_t resIdxN = 0U;
         for (; resIdxN < 16U; resIdxN++)
-            t_tile[(blockIdx.x / (cols / 32U) * 32U + threadIdx.x / 2U * 16U +
-                    resIdxM) * cols + blockIdx.x % (cols / 32U) * 32U +
-                   threadIdx.x % 2U * 16U + resIdxN]
+            t_tile[(32U * (blockIdx.x / (cols / 32U)) +
+                    16U * (threadIdx.x / 2U) + resIdxM) * cols +
+                   32U * (blockIdx.x % (cols / 32U)) +
+                   16U * (threadIdx.x % 2U) + resIdxN]
                 = beta *
-                t_tile[(blockIdx.x / (cols / 32U) * 32U +
-                        threadIdx.x / 2U * 16U + resIdxM) * cols +
-                       blockIdx.x % (cols / 32U) * 32U +
-                       threadIdx.x % 2U * 16U + resIdxN]
+                t_tile[(32U * (blockIdx.x / (cols / 32U)) +
+                        16U * (threadIdx.x / 2U) + resIdxM) * cols +
+                       32U * (blockIdx.x % (cols / 32U)) +
+                       16U * (threadIdx.x % 2U) + resIdxN]
                 + alpha * rchProd[resIdxM * 16U + resIdxN];
     }
 }
@@ -897,6 +913,7 @@ __hoisted_8(float alpha,
             for (; k < 4U; k++)
                 sA[(col + k) * 32U + row] = local[k];
         }
+        uint32_t __anf06 = bkIdx;
         float *tileB = gB;
         uint32_t i = 0U;
         for (; i < 2048U; i += 128U) {
@@ -905,7 +922,7 @@ __hoisted_8(float alpha,
             uint32_t row = (i + threadIdx.x * 4U) / 64U;
             uint32_t col = (i + threadIdx.x * 4U) % 64U;
             vec_memcpy(local,
-                       tileB + cols * (__anf03 * 32U) + mcol * 64U +
+                       tileB + cols * (__anf06 * 32U) + mcol * 64U +
                        cols * row + col);
             uint32_t k = 0U;
             for (; k < 4U; k++)
@@ -939,14 +956,15 @@ __hoisted_8(float alpha,
     for (; resIdxM < 8U; resIdxM++) {
         uint32_t resIdxN = 0U;
         for (; resIdxN < 8U; resIdxN++)
-            t_tile[(blockIdx.x / (cols / 64U) * 32U + threadIdx.x / 8U * 8U +
-                    resIdxM) * cols + blockIdx.x % (cols / 64U) * 64U +
-                   threadIdx.x % 8U * 8U + resIdxN]
+            t_tile[(32U * (blockIdx.x / (cols / 64U)) +
+                    8U * (threadIdx.x / 8U) + resIdxM) * cols +
+                   64U * (blockIdx.x % (cols / 64U)) + 8U * (threadIdx.x % 8U) +
+                   resIdxN]
                 = beta *
-                t_tile[(blockIdx.x / (cols / 64U) * 32U +
-                        threadIdx.x / 8U * 8U + resIdxM) * cols +
-                       blockIdx.x % (cols / 64U) * 64U + threadIdx.x % 8U * 8U +
-                       resIdxN]
+                t_tile[(32U * (blockIdx.x / (cols / 64U)) +
+                        8U * (threadIdx.x / 8U) + resIdxM) * cols +
+                       64U * (blockIdx.x % (cols / 64U)) +
+                       8U * (threadIdx.x % 8U) + resIdxN]
                 + alpha * rchProd[resIdxM * 8U + resIdxN];
     }
 }
@@ -1004,6 +1022,7 @@ __hoisted_9(float alpha,
             for (; k < 4U; k++)
                 sA[(col + k) * 32U + row] = local[k];
         }
+        uint32_t __anf06 = bkIdx;
         float *tileB = gB;
         uint32_t i = 0U;
         for (; i < 2048U; i += 64U) {
@@ -1012,7 +1031,7 @@ __hoisted_9(float alpha,
             uint32_t row = (i + threadIdx.x * 4U) / 64U;
             uint32_t col = (i + threadIdx.x * 4U) % 64U;
             vec_memcpy(local,
-                       tileB + cols * (__anf03 * 32U) + mcol * 64U +
+                       tileB + cols * (__anf06 * 32U) + mcol * 64U +
                        cols * row + col);
             uint32_t k = 0U;
             for (; k < 4U; k++)
@@ -1046,14 +1065,15 @@ __hoisted_9(float alpha,
     for (; resIdxM < 8U; resIdxM++) {
         uint32_t resIdxN = 0U;
         for (; resIdxN < 16U; resIdxN++)
-            t_tile[(blockIdx.x / (cols / 64U) * 32U + threadIdx.x / 4U * 8U +
-                    resIdxM) * cols + blockIdx.x % (cols / 64U) * 64U +
-                   threadIdx.x % 4U * 16U + resIdxN]
+            t_tile[(32U * (blockIdx.x / (cols / 64U)) +
+                    8U * (threadIdx.x / 4U) + resIdxM) * cols +
+                   64U * (blockIdx.x % (cols / 64U)) +
+                   16U * (threadIdx.x % 4U) + resIdxN]
                 = beta *
-                t_tile[(blockIdx.x / (cols / 64U) * 32U +
-                        threadIdx.x / 4U * 8U + resIdxM) * cols +
-                       blockIdx.x % (cols / 64U) * 64U +
-                       threadIdx.x % 4U * 16U + resIdxN]
+                t_tile[(32U * (blockIdx.x / (cols / 64U)) +
+                        8U * (threadIdx.x / 4U) + resIdxM) * cols +
+                       64U * (blockIdx.x % (cols / 64U)) +
+                       16U * (threadIdx.x % 4U) + resIdxN]
                 + alpha * rchProd[resIdxM * 16U + resIdxN];
     }
 }
@@ -1112,6 +1132,7 @@ __hoisted_10(float alpha,
             for (; k < 4U; k++)
                 sA[(col + k) * 32U + row] = local[k];
         }
+        uint32_t __anf06 = bkIdx;
         float *tileB = gB;
         uint32_t i = 0U;
         for (; i < 2048U; i += 64U) {
@@ -1120,7 +1141,7 @@ __hoisted_10(float alpha,
             uint32_t row = (i + threadIdx.x * 4U) / 64U;
             uint32_t col = (i + threadIdx.x * 4U) % 64U;
             vec_memcpy(local,
-                       tileB + cols * (__anf03 * 32U) + mcol * 64U +
+                       tileB + cols * (__anf06 * 32U) + mcol * 64U +
                        cols * row + col);
             uint32_t k = 0U;
             for (; k < 4U; k++)
@@ -1154,14 +1175,15 @@ __hoisted_10(float alpha,
     for (; resIdxM < 16U; resIdxM++) {
         uint32_t resIdxN = 0U;
         for (; resIdxN < 8U; resIdxN++)
-            t_tile[(blockIdx.x / (cols / 64U) * 32U + threadIdx.x / 8U * 16U +
-                    resIdxM) * cols + blockIdx.x % (cols / 64U) * 64U +
-                   threadIdx.x % 8U * 8U + resIdxN]
+            t_tile[(32U * (blockIdx.x / (cols / 64U)) +
+                    16U * (threadIdx.x / 8U) + resIdxM) * cols +
+                   64U * (blockIdx.x % (cols / 64U)) + 8U * (threadIdx.x % 8U) +
+                   resIdxN]
                 = beta *
-                t_tile[(blockIdx.x / (cols / 64U) * 32U +
-                        threadIdx.x / 8U * 16U + resIdxM) * cols +
-                       blockIdx.x % (cols / 64U) * 64U + threadIdx.x % 8U * 8U +
-                       resIdxN]
+                t_tile[(32U * (blockIdx.x / (cols / 64U)) +
+                        16U * (threadIdx.x / 8U) + resIdxM) * cols +
+                       64U * (blockIdx.x % (cols / 64U)) +
+                       8U * (threadIdx.x % 8U) + resIdxN]
                 + alpha * rchProd[resIdxM * 8U + resIdxN];
     }
 }
@@ -1220,6 +1242,7 @@ __hoisted_11(float alpha,
             for (; k < 4U; k++)
                 sA[(col + k) * 32U + row] = local[k];
         }
+        uint32_t __anf06 = bkIdx;
         float *tileB = gB;
         uint32_t i = 0U;
         for (; i < 2048U; i += 32U) {
@@ -1228,7 +1251,7 @@ __hoisted_11(float alpha,
             uint32_t row = (i + threadIdx.x * 4U) / 64U;
             uint32_t col = (i + threadIdx.x * 4U) % 64U;
             vec_memcpy(local,
-                       tileB + cols * (__anf03 * 32U) + mcol * 64U +
+                       tileB + cols * (__anf06 * 32U) + mcol * 64U +
                        cols * row + col);
             uint32_t k = 0U;
             for (; k < 4U; k++)
@@ -1262,14 +1285,15 @@ __hoisted_11(float alpha,
     for (; resIdxM < 16U; resIdxM++) {
         uint32_t resIdxN = 0U;
         for (; resIdxN < 16U; resIdxN++)
-            t_tile[(blockIdx.x / (cols / 64U) * 32U + threadIdx.x / 4U * 16U +
-                    resIdxM) * cols + blockIdx.x % (cols / 64U) * 64U +
-                   threadIdx.x % 4U * 16U + resIdxN]
+            t_tile[(32U * (blockIdx.x / (cols / 64U)) +
+                    16U * (threadIdx.x / 4U) + resIdxM) * cols +
+                   64U * (blockIdx.x % (cols / 64U)) +
+                   16U * (threadIdx.x % 4U) + resIdxN]
                 = beta *
-                t_tile[(blockIdx.x / (cols / 64U) * 32U +
-                        threadIdx.x / 4U * 16U + resIdxM) * cols +
-                       blockIdx.x % (cols / 64U) * 64U +
-                       threadIdx.x % 4U * 16U + resIdxN]
+                t_tile[(32U * (blockIdx.x / (cols / 64U)) +
+                        16U * (threadIdx.x / 4U) + resIdxM) * cols +
+                       64U * (blockIdx.x % (cols / 64U)) +
+                       16U * (threadIdx.x % 4U) + resIdxN]
                 + alpha * rchProd[resIdxM * 16U + resIdxN];
     }
 }
@@ -1328,6 +1352,7 @@ __hoisted_12(float alpha,
             for (; k < 4U; k++)
                 sA[(col + k) * 32U + row] = local[k];
         }
+        uint32_t __anf06 = bkIdx;
         float *tileB = gB;
         uint32_t i = 0U;
         for (; i < 4096U; i += 128U) {
@@ -1336,7 +1361,7 @@ __hoisted_12(float alpha,
             uint32_t row = (i + threadIdx.x * 4U) / 64U;
             uint32_t col = (i + threadIdx.x * 4U) % 64U;
             vec_memcpy(local,
-                       tileB + cols * (__anf03 * 64U) + mcol * 64U +
+                       tileB + cols * (__anf06 * 64U) + mcol * 64U +
                        cols * row + col);
             uint32_t k = 0U;
             for (; k < 4U; k++)
@@ -1370,14 +1395,15 @@ __hoisted_12(float alpha,
     for (; resIdxM < 8U; resIdxM++) {
         uint32_t resIdxN = 0U;
         for (; resIdxN < 8U; resIdxN++)
-            t_tile[(blockIdx.x / (cols / 64U) * 32U + threadIdx.x / 8U * 8U +
-                    resIdxM) * cols + blockIdx.x % (cols / 64U) * 64U +
-                   threadIdx.x % 8U * 8U + resIdxN]
+            t_tile[(32U * (blockIdx.x / (cols / 64U)) +
+                    8U * (threadIdx.x / 8U) + resIdxM) * cols +
+                   64U * (blockIdx.x % (cols / 64U)) + 8U * (threadIdx.x % 8U) +
+                   resIdxN]
                 = beta *
-                t_tile[(blockIdx.x / (cols / 64U) * 32U +
-                        threadIdx.x / 8U * 8U + resIdxM) * cols +
-                       blockIdx.x % (cols / 64U) * 64U + threadIdx.x % 8U * 8U +
-                       resIdxN]
+                t_tile[(32U * (blockIdx.x / (cols / 64U)) +
+                        8U * (threadIdx.x / 8U) + resIdxM) * cols +
+                       64U * (blockIdx.x % (cols / 64U)) +
+                       8U * (threadIdx.x % 8U) + resIdxN]
                 + alpha * rchProd[resIdxM * 8U + resIdxN];
     }
 }
@@ -1435,6 +1461,7 @@ __hoisted_13(float alpha,
             for (; k < 4U; k++)
                 sA[(col + k) * 32U + row] = local[k];
         }
+        uint32_t __anf06 = bkIdx;
         float *tileB = gB;
         uint32_t i = 0U;
         for (; i < 4096U; i += 64U) {
@@ -1443,7 +1470,7 @@ __hoisted_13(float alpha,
             uint32_t row = (i + threadIdx.x * 4U) / 64U;
             uint32_t col = (i + threadIdx.x * 4U) % 64U;
             vec_memcpy(local,
-                       tileB + cols * (__anf03 * 64U) + mcol * 64U +
+                       tileB + cols * (__anf06 * 64U) + mcol * 64U +
                        cols * row + col);
             uint32_t k = 0U;
             for (; k < 4U; k++)
@@ -1477,14 +1504,15 @@ __hoisted_13(float alpha,
     for (; resIdxM < 8U; resIdxM++) {
         uint32_t resIdxN = 0U;
         for (; resIdxN < 16U; resIdxN++)
-            t_tile[(blockIdx.x / (cols / 64U) * 32U + threadIdx.x / 4U * 8U +
-                    resIdxM) * cols + blockIdx.x % (cols / 64U) * 64U +
-                   threadIdx.x % 4U * 16U + resIdxN]
+            t_tile[(32U * (blockIdx.x / (cols / 64U)) +
+                    8U * (threadIdx.x / 4U) + resIdxM) * cols +
+                   64U * (blockIdx.x % (cols / 64U)) +
+                   16U * (threadIdx.x % 4U) + resIdxN]
                 = beta *
-                t_tile[(blockIdx.x / (cols / 64U) * 32U +
-                        threadIdx.x / 4U * 8U + resIdxM) * cols +
-                       blockIdx.x % (cols / 64U) * 64U +
-                       threadIdx.x % 4U * 16U + resIdxN]
+                t_tile[(32U * (blockIdx.x / (cols / 64U)) +
+                        8U * (threadIdx.x / 4U) + resIdxM) * cols +
+                       64U * (blockIdx.x % (cols / 64U)) +
+                       16U * (threadIdx.x % 4U) + resIdxN]
                 + alpha * rchProd[resIdxM * 16U + resIdxN];
     }
 }
@@ -1543,6 +1571,7 @@ __hoisted_14(float alpha,
             for (; k < 4U; k++)
                 sA[(col + k) * 32U + row] = local[k];
         }
+        uint32_t __anf06 = bkIdx;
         float *tileB = gB;
         uint32_t i = 0U;
         for (; i < 4096U; i += 64U) {
@@ -1551,7 +1580,7 @@ __hoisted_14(float alpha,
             uint32_t row = (i + threadIdx.x * 4U) / 64U;
             uint32_t col = (i + threadIdx.x * 4U) % 64U;
             vec_memcpy(local,
-                       tileB + cols * (__anf03 * 64U) + mcol * 64U +
+                       tileB + cols * (__anf06 * 64U) + mcol * 64U +
                        cols * row + col);
             uint32_t k = 0U;
             for (; k < 4U; k++)
@@ -1585,14 +1614,15 @@ __hoisted_14(float alpha,
     for (; resIdxM < 16U; resIdxM++) {
         uint32_t resIdxN = 0U;
         for (; resIdxN < 8U; resIdxN++)
-            t_tile[(blockIdx.x / (cols / 64U) * 32U + threadIdx.x / 8U * 16U +
-                    resIdxM) * cols + blockIdx.x % (cols / 64U) * 64U +
-                   threadIdx.x % 8U * 8U + resIdxN]
+            t_tile[(32U * (blockIdx.x / (cols / 64U)) +
+                    16U * (threadIdx.x / 8U) + resIdxM) * cols +
+                   64U * (blockIdx.x % (cols / 64U)) + 8U * (threadIdx.x % 8U) +
+                   resIdxN]
                 = beta *
-                t_tile[(blockIdx.x / (cols / 64U) * 32U +
-                        threadIdx.x / 8U * 16U + resIdxM) * cols +
-                       blockIdx.x % (cols / 64U) * 64U + threadIdx.x % 8U * 8U +
-                       resIdxN]
+                t_tile[(32U * (blockIdx.x / (cols / 64U)) +
+                        16U * (threadIdx.x / 8U) + resIdxM) * cols +
+                       64U * (blockIdx.x % (cols / 64U)) +
+                       8U * (threadIdx.x % 8U) + resIdxN]
                 + alpha * rchProd[resIdxM * 8U + resIdxN];
     }
 }
@@ -1651,6 +1681,7 @@ __hoisted_15(float alpha,
             for (; k < 4U; k++)
                 sA[(col + k) * 32U + row] = local[k];
         }
+        uint32_t __anf06 = bkIdx;
         float *tileB = gB;
         uint32_t i = 0U;
         for (; i < 4096U; i += 32U) {
@@ -1659,7 +1690,7 @@ __hoisted_15(float alpha,
             uint32_t row = (i + threadIdx.x * 4U) / 64U;
             uint32_t col = (i + threadIdx.x * 4U) % 64U;
             vec_memcpy(local,
-                       tileB + cols * (__anf03 * 64U) + mcol * 64U +
+                       tileB + cols * (__anf06 * 64U) + mcol * 64U +
                        cols * row + col);
             uint32_t k = 0U;
             for (; k < 4U; k++)
@@ -1693,14 +1724,15 @@ __hoisted_15(float alpha,
     for (; resIdxM < 16U; resIdxM++) {
         uint32_t resIdxN = 0U;
         for (; resIdxN < 16U; resIdxN++)
-            t_tile[(blockIdx.x / (cols / 64U) * 32U + threadIdx.x / 4U * 16U +
-                    resIdxM) * cols + blockIdx.x % (cols / 64U) * 64U +
-                   threadIdx.x % 4U * 16U + resIdxN]
+            t_tile[(32U * (blockIdx.x / (cols / 64U)) +
+                    16U * (threadIdx.x / 4U) + resIdxM) * cols +
+                   64U * (blockIdx.x % (cols / 64U)) +
+                   16U * (threadIdx.x % 4U) + resIdxN]
                 = beta *
-                t_tile[(blockIdx.x / (cols / 64U) * 32U +
-                        threadIdx.x / 4U * 16U + resIdxM) * cols +
-                       blockIdx.x % (cols / 64U) * 64U +
-                       threadIdx.x % 4U * 16U + resIdxN]
+                t_tile[(32U * (blockIdx.x / (cols / 64U)) +
+                        16U * (threadIdx.x / 4U) + resIdxM) * cols +
+                       64U * (blockIdx.x % (cols / 64U)) +
+                       16U * (threadIdx.x % 4U) + resIdxN]
                 + alpha * rchProd[resIdxM * 16U + resIdxN];
     }
 }
@@ -1759,6 +1791,7 @@ __hoisted_16(float alpha,
             for (; k < 4U; k++)
                 sA[(col + k) * 32U + row] = local[k];
         }
+        uint32_t __anf06 = bkIdx;
         float *tileB = gB;
         uint32_t i = 0U;
         for (; i < 4096U; i += 256U) {
@@ -1767,7 +1800,7 @@ __hoisted_16(float alpha,
             uint32_t row = (i + threadIdx.x * 4U) / 128U;
             uint32_t col = (i + threadIdx.x * 4U) % 128U;
             vec_memcpy(local,
-                       tileB + cols * (__anf03 * 32U) + mcol * 128U +
+                       tileB + cols * (__anf06 * 32U) + mcol * 128U +
                        cols * row + col);
             uint32_t k = 0U;
             for (; k < 4U; k++)
@@ -1801,14 +1834,15 @@ __hoisted_16(float alpha,
     for (; resIdxM < 8U; resIdxM++) {
         uint32_t resIdxN = 0U;
         for (; resIdxN < 8U; resIdxN++)
-            t_tile[(blockIdx.x / (cols / 128U) * 32U + threadIdx.x / 16U * 8U +
-                    resIdxM) * cols + blockIdx.x % (cols / 128U) * 128U +
-                   threadIdx.x % 16U * 8U + resIdxN]
+            t_tile[(32U * (blockIdx.x / (cols / 128U)) +
+                    8U * (threadIdx.x / 16U) + resIdxM) * cols +
+                   128U * (blockIdx.x % (cols / 128U)) +
+                   8U * (threadIdx.x % 16U) + resIdxN]
                 = beta *
-                t_tile[(blockIdx.x / (cols / 128U) * 32U +
-                        threadIdx.x / 16U * 8U + resIdxM) * cols +
-                       blockIdx.x % (cols / 128U) * 128U +
-                       threadIdx.x % 16U * 8U + resIdxN]
+                t_tile[(32U * (blockIdx.x / (cols / 128U)) +
+                        8U * (threadIdx.x / 16U) + resIdxM) * cols +
+                       128U * (blockIdx.x % (cols / 128U)) +
+                       8U * (threadIdx.x % 16U) + resIdxN]
                 + alpha * rchProd[resIdxM * 8U + resIdxN];
     }
 }
@@ -1867,6 +1901,7 @@ __hoisted_17(float alpha,
             for (; k < 4U; k++)
                 sA[(col + k) * 32U + row] = local[k];
         }
+        uint32_t __anf06 = bkIdx;
         float *tileB = gB;
         uint32_t i = 0U;
         for (; i < 4096U; i += 128U) {
@@ -1875,7 +1910,7 @@ __hoisted_17(float alpha,
             uint32_t row = (i + threadIdx.x * 4U) / 128U;
             uint32_t col = (i + threadIdx.x * 4U) % 128U;
             vec_memcpy(local,
-                       tileB + cols * (__anf03 * 32U) + mcol * 128U +
+                       tileB + cols * (__anf06 * 32U) + mcol * 128U +
                        cols * row + col);
             uint32_t k = 0U;
             for (; k < 4U; k++)
@@ -1909,14 +1944,15 @@ __hoisted_17(float alpha,
     for (; resIdxM < 8U; resIdxM++) {
         uint32_t resIdxN = 0U;
         for (; resIdxN < 16U; resIdxN++)
-            t_tile[(blockIdx.x / (cols / 128U) * 32U + threadIdx.x / 8U * 8U +
-                    resIdxM) * cols + blockIdx.x % (cols / 128U) * 128U +
-                   threadIdx.x % 8U * 16U + resIdxN]
+            t_tile[(32U * (blockIdx.x / (cols / 128U)) +
+                    8U * (threadIdx.x / 8U) + resIdxM) * cols +
+                   128U * (blockIdx.x % (cols / 128U)) +
+                   16U * (threadIdx.x % 8U) + resIdxN]
                 = beta *
-                t_tile[(blockIdx.x / (cols / 128U) * 32U +
-                        threadIdx.x / 8U * 8U + resIdxM) * cols +
-                       blockIdx.x % (cols / 128U) * 128U +
-                       threadIdx.x % 8U * 16U + resIdxN]
+                t_tile[(32U * (blockIdx.x / (cols / 128U)) +
+                        8U * (threadIdx.x / 8U) + resIdxM) * cols +
+                       128U * (blockIdx.x % (cols / 128U)) +
+                       16U * (threadIdx.x % 8U) + resIdxN]
                 + alpha * rchProd[resIdxM * 16U + resIdxN];
     }
 }
@@ -1975,6 +2011,7 @@ __hoisted_18(float alpha,
             for (; k < 4U; k++)
                 sA[(col + k) * 32U + row] = local[k];
         }
+        uint32_t __anf06 = bkIdx;
         float *tileB = gB;
         uint32_t i = 0U;
         for (; i < 4096U; i += 128U) {
@@ -1983,7 +2020,7 @@ __hoisted_18(float alpha,
             uint32_t row = (i + threadIdx.x * 4U) / 128U;
             uint32_t col = (i + threadIdx.x * 4U) % 128U;
             vec_memcpy(local,
-                       tileB + cols * (__anf03 * 32U) + mcol * 128U +
+                       tileB + cols * (__anf06 * 32U) + mcol * 128U +
                        cols * row + col);
             uint32_t k = 0U;
             for (; k < 4U; k++)
@@ -2017,14 +2054,15 @@ __hoisted_18(float alpha,
     for (; resIdxM < 16U; resIdxM++) {
         uint32_t resIdxN = 0U;
         for (; resIdxN < 8U; resIdxN++)
-            t_tile[(blockIdx.x / (cols / 128U) * 32U + threadIdx.x / 16U * 16U +
-                    resIdxM) * cols + blockIdx.x % (cols / 128U) * 128U +
-                   threadIdx.x % 16U * 8U + resIdxN]
+            t_tile[(32U * (blockIdx.x / (cols / 128U)) +
+                    16U * (threadIdx.x / 16U) + resIdxM) * cols +
+                   128U * (blockIdx.x % (cols / 128U)) +
+                   8U * (threadIdx.x % 16U) + resIdxN]
                 = beta *
-                t_tile[(blockIdx.x / (cols / 128U) * 32U +
-                        threadIdx.x / 16U * 16U + resIdxM) * cols +
-                       blockIdx.x % (cols / 128U) * 128U +
-                       threadIdx.x % 16U * 8U + resIdxN]
+                t_tile[(32U * (blockIdx.x / (cols / 128U)) +
+                        16U * (threadIdx.x / 16U) + resIdxM) * cols +
+                       128U * (blockIdx.x % (cols / 128U)) +
+                       8U * (threadIdx.x % 16U) + resIdxN]
                 + alpha * rchProd[resIdxM * 8U + resIdxN];
     }
 }
@@ -2083,6 +2121,7 @@ __hoisted_19(float alpha,
             for (; k < 4U; k++)
                 sA[(col + k) * 32U + row] = local[k];
         }
+        uint32_t __anf06 = bkIdx;
         float *tileB = gB;
         uint32_t i = 0U;
         for (; i < 4096U; i += 64U) {
@@ -2091,7 +2130,7 @@ __hoisted_19(float alpha,
             uint32_t row = (i + threadIdx.x * 4U) / 128U;
             uint32_t col = (i + threadIdx.x * 4U) % 128U;
             vec_memcpy(local,
-                       tileB + cols * (__anf03 * 32U) + mcol * 128U +
+                       tileB + cols * (__anf06 * 32U) + mcol * 128U +
                        cols * row + col);
             uint32_t k = 0U;
             for (; k < 4U; k++)
@@ -2125,14 +2164,15 @@ __hoisted_19(float alpha,
     for (; resIdxM < 16U; resIdxM++) {
         uint32_t resIdxN = 0U;
         for (; resIdxN < 16U; resIdxN++)
-            t_tile[(blockIdx.x / (cols / 128U) * 32U + threadIdx.x / 8U * 16U +
-                    resIdxM) * cols + blockIdx.x % (cols / 128U) * 128U +
-                   threadIdx.x % 8U * 16U + resIdxN]
+            t_tile[(32U * (blockIdx.x / (cols / 128U)) +
+                    16U * (threadIdx.x / 8U) + resIdxM) * cols +
+                   128U * (blockIdx.x % (cols / 128U)) +
+                   16U * (threadIdx.x % 8U) + resIdxN]
                 = beta *
-                t_tile[(blockIdx.x / (cols / 128U) * 32U +
-                        threadIdx.x / 8U * 16U + resIdxM) * cols +
-                       blockIdx.x % (cols / 128U) * 128U +
-                       threadIdx.x % 8U * 16U + resIdxN]
+                t_tile[(32U * (blockIdx.x / (cols / 128U)) +
+                        16U * (threadIdx.x / 8U) + resIdxM) * cols +
+                       128U * (blockIdx.x % (cols / 128U)) +
+                       16U * (threadIdx.x % 8U) + resIdxN]
                 + alpha * rchProd[resIdxM * 16U + resIdxN];
     }
 }
@@ -2191,6 +2231,7 @@ __hoisted_20(float alpha,
             for (; k < 4U; k++)
                 sA[(col + k) * 32U + row] = local[k];
         }
+        uint32_t __anf06 = bkIdx;
         float *tileB = gB;
         uint32_t i = 0U;
         for (; i < 8192U; i += 256U) {
@@ -2199,7 +2240,7 @@ __hoisted_20(float alpha,
             uint32_t row = (i + threadIdx.x * 4U) / 128U;
             uint32_t col = (i + threadIdx.x * 4U) % 128U;
             vec_memcpy(local,
-                       tileB + cols * (__anf03 * 64U) + mcol * 128U +
+                       tileB + cols * (__anf06 * 64U) + mcol * 128U +
                        cols * row + col);
             uint32_t k = 0U;
             for (; k < 4U; k++)
@@ -2233,14 +2274,15 @@ __hoisted_20(float alpha,
     for (; resIdxM < 8U; resIdxM++) {
         uint32_t resIdxN = 0U;
         for (; resIdxN < 8U; resIdxN++)
-            t_tile[(blockIdx.x / (cols / 128U) * 32U + threadIdx.x / 16U * 8U +
-                    resIdxM) * cols + blockIdx.x % (cols / 128U) * 128U +
-                   threadIdx.x % 16U * 8U + resIdxN]
+            t_tile[(32U * (blockIdx.x / (cols / 128U)) +
+                    8U * (threadIdx.x / 16U) + resIdxM) * cols +
+                   128U * (blockIdx.x % (cols / 128U)) +
+                   8U * (threadIdx.x % 16U) + resIdxN]
                 = beta *
-                t_tile[(blockIdx.x / (cols / 128U) * 32U +
-                        threadIdx.x / 16U * 8U + resIdxM) * cols +
-                       blockIdx.x % (cols / 128U) * 128U +
-                       threadIdx.x % 16U * 8U + resIdxN]
+                t_tile[(32U * (blockIdx.x / (cols / 128U)) +
+                        8U * (threadIdx.x / 16U) + resIdxM) * cols +
+                       128U * (blockIdx.x % (cols / 128U)) +
+                       8U * (threadIdx.x % 16U) + resIdxN]
                 + alpha * rchProd[resIdxM * 8U + resIdxN];
     }
 }
@@ -2299,6 +2341,7 @@ __hoisted_21(float alpha,
             for (; k < 4U; k++)
                 sA[(col + k) * 32U + row] = local[k];
         }
+        uint32_t __anf06 = bkIdx;
         float *tileB = gB;
         uint32_t i = 0U;
         for (; i < 8192U; i += 128U) {
@@ -2307,7 +2350,7 @@ __hoisted_21(float alpha,
             uint32_t row = (i + threadIdx.x * 4U) / 128U;
             uint32_t col = (i + threadIdx.x * 4U) % 128U;
             vec_memcpy(local,
-                       tileB + cols * (__anf03 * 64U) + mcol * 128U +
+                       tileB + cols * (__anf06 * 64U) + mcol * 128U +
                        cols * row + col);
             uint32_t k = 0U;
             for (; k < 4U; k++)
@@ -2341,14 +2384,15 @@ __hoisted_21(float alpha,
     for (; resIdxM < 8U; resIdxM++) {
         uint32_t resIdxN = 0U;
         for (; resIdxN < 16U; resIdxN++)
-            t_tile[(blockIdx.x / (cols / 128U) * 32U + threadIdx.x / 8U * 8U +
-                    resIdxM) * cols + blockIdx.x % (cols / 128U) * 128U +
-                   threadIdx.x % 8U * 16U + resIdxN]
+            t_tile[(32U * (blockIdx.x / (cols / 128U)) +
+                    8U * (threadIdx.x / 8U) + resIdxM) * cols +
+                   128U * (blockIdx.x % (cols / 128U)) +
+                   16U * (threadIdx.x % 8U) + resIdxN]
                 = beta *
-                t_tile[(blockIdx.x / (cols / 128U) * 32U +
-                        threadIdx.x / 8U * 8U + resIdxM) * cols +
-                       blockIdx.x % (cols / 128U) * 128U +
-                       threadIdx.x % 8U * 16U + resIdxN]
+                t_tile[(32U * (blockIdx.x / (cols / 128U)) +
+                        8U * (threadIdx.x / 8U) + resIdxM) * cols +
+                       128U * (blockIdx.x % (cols / 128U)) +
+                       16U * (threadIdx.x % 8U) + resIdxN]
                 + alpha * rchProd[resIdxM * 16U + resIdxN];
     }
 }
@@ -2407,6 +2451,7 @@ __hoisted_22(float alpha,
             for (; k < 4U; k++)
                 sA[(col + k) * 32U + row] = local[k];
         }
+        uint32_t __anf06 = bkIdx;
         float *tileB = gB;
         uint32_t i = 0U;
         for (; i < 8192U; i += 128U) {
@@ -2415,7 +2460,7 @@ __hoisted_22(float alpha,
             uint32_t row = (i + threadIdx.x * 4U) / 128U;
             uint32_t col = (i + threadIdx.x * 4U) % 128U;
             vec_memcpy(local,
-                       tileB + cols * (__anf03 * 64U) + mcol * 128U +
+                       tileB + cols * (__anf06 * 64U) + mcol * 128U +
                        cols * row + col);
             uint32_t k = 0U;
             for (; k < 4U; k++)
@@ -2449,14 +2494,15 @@ __hoisted_22(float alpha,
     for (; resIdxM < 16U; resIdxM++) {
         uint32_t resIdxN = 0U;
         for (; resIdxN < 8U; resIdxN++)
-            t_tile[(blockIdx.x / (cols / 128U) * 32U + threadIdx.x / 16U * 16U +
-                    resIdxM) * cols + blockIdx.x % (cols / 128U) * 128U +
-                   threadIdx.x % 16U * 8U + resIdxN]
+            t_tile[(32U * (blockIdx.x / (cols / 128U)) +
+                    16U * (threadIdx.x / 16U) + resIdxM) * cols +
+                   128U * (blockIdx.x % (cols / 128U)) +
+                   8U * (threadIdx.x % 16U) + resIdxN]
                 = beta *
-                t_tile[(blockIdx.x / (cols / 128U) * 32U +
-                        threadIdx.x / 16U * 16U + resIdxM) * cols +
-                       blockIdx.x % (cols / 128U) * 128U +
-                       threadIdx.x % 16U * 8U + resIdxN]
+                t_tile[(32U * (blockIdx.x / (cols / 128U)) +
+                        16U * (threadIdx.x / 16U) + resIdxM) * cols +
+                       128U * (blockIdx.x % (cols / 128U)) +
+                       8U * (threadIdx.x % 16U) + resIdxN]
                 + alpha * rchProd[resIdxM * 8U + resIdxN];
     }
 }
@@ -2515,6 +2561,7 @@ __hoisted_23(float alpha,
             for (; k < 4U; k++)
                 sA[(col + k) * 32U + row] = local[k];
         }
+        uint32_t __anf06 = bkIdx;
         float *tileB = gB;
         uint32_t i = 0U;
         for (; i < 8192U; i += 64U) {
@@ -2523,7 +2570,7 @@ __hoisted_23(float alpha,
             uint32_t row = (i + threadIdx.x * 4U) / 128U;
             uint32_t col = (i + threadIdx.x * 4U) % 128U;
             vec_memcpy(local,
-                       tileB + cols * (__anf03 * 64U) + mcol * 128U +
+                       tileB + cols * (__anf06 * 64U) + mcol * 128U +
                        cols * row + col);
             uint32_t k = 0U;
             for (; k < 4U; k++)
@@ -2557,14 +2604,15 @@ __hoisted_23(float alpha,
     for (; resIdxM < 16U; resIdxM++) {
         uint32_t resIdxN = 0U;
         for (; resIdxN < 16U; resIdxN++)
-            t_tile[(blockIdx.x / (cols / 128U) * 32U + threadIdx.x / 8U * 16U +
-                    resIdxM) * cols + blockIdx.x % (cols / 128U) * 128U +
-                   threadIdx.x % 8U * 16U + resIdxN]
+            t_tile[(32U * (blockIdx.x / (cols / 128U)) +
+                    16U * (threadIdx.x / 8U) + resIdxM) * cols +
+                   128U * (blockIdx.x % (cols / 128U)) +
+                   16U * (threadIdx.x % 8U) + resIdxN]
                 = beta *
-                t_tile[(blockIdx.x / (cols / 128U) * 32U +
-                        threadIdx.x / 8U * 16U + resIdxM) * cols +
-                       blockIdx.x % (cols / 128U) * 128U +
-                       threadIdx.x % 8U * 16U + resIdxN]
+                t_tile[(32U * (blockIdx.x / (cols / 128U)) +
+                        16U * (threadIdx.x / 8U) + resIdxM) * cols +
+                       128U * (blockIdx.x % (cols / 128U)) +
+                       16U * (threadIdx.x % 8U) + resIdxN]
                 + alpha * rchProd[resIdxM * 16U + resIdxN];
     }
 }
@@ -2623,6 +2671,7 @@ __hoisted_24(float alpha,
             for (; k < 4U; k++)
                 sA[(col + k) * 64U + row] = local[k];
         }
+        uint32_t __anf06 = bkIdx;
         float *tileB = gB;
         uint32_t i = 0U;
         for (; i < 1024U; i += 128U) {
@@ -2631,7 +2680,7 @@ __hoisted_24(float alpha,
             uint32_t row = (i + threadIdx.x * 4U) / 32U;
             uint32_t col = (i + threadIdx.x * 4U) % 32U;
             vec_memcpy(local,
-                       tileB + cols * (__anf03 * 32U) + mcol * 32U +
+                       tileB + cols * (__anf06 * 32U) + mcol * 32U +
                        cols * row + col);
             uint32_t k = 0U;
             for (; k < 4U; k++)
@@ -2665,14 +2714,15 @@ __hoisted_24(float alpha,
     for (; resIdxM < 8U; resIdxM++) {
         uint32_t resIdxN = 0U;
         for (; resIdxN < 8U; resIdxN++)
-            t_tile[(blockIdx.x / (cols / 32U) * 64U + threadIdx.x / 4U * 8U +
-                    resIdxM) * cols + blockIdx.x % (cols / 32U) * 32U +
-                   threadIdx.x % 4U * 8U + resIdxN]
+            t_tile[(64U * (blockIdx.x / (cols / 32U)) +
+                    8U * (threadIdx.x / 4U) + resIdxM) * cols +
+                   32U * (blockIdx.x % (cols / 32U)) + 8U * (threadIdx.x % 4U) +
+                   resIdxN]
                 = beta *
-                t_tile[(blockIdx.x / (cols / 32U) * 64U +
-                        threadIdx.x / 4U * 8U + resIdxM) * cols +
-                       blockIdx.x % (cols / 32U) * 32U + threadIdx.x % 4U * 8U +
-                       resIdxN]
+                t_tile[(64U * (blockIdx.x / (cols / 32U)) +
+                        8U * (threadIdx.x / 4U) + resIdxM) * cols +
+                       32U * (blockIdx.x % (cols / 32U)) +
+                       8U * (threadIdx.x % 4U) + resIdxN]
                 + alpha * rchProd[resIdxM * 8U + resIdxN];
     }
 }
@@ -2730,6 +2780,7 @@ __hoisted_25(float alpha,
             for (; k < 4U; k++)
                 sA[(col + k) * 64U + row] = local[k];
         }
+        uint32_t __anf06 = bkIdx;
         float *tileB = gB;
         uint32_t i = 0U;
         for (; i < 1024U; i += 64U) {
@@ -2738,7 +2789,7 @@ __hoisted_25(float alpha,
             uint32_t row = (i + threadIdx.x * 4U) / 32U;
             uint32_t col = (i + threadIdx.x * 4U) % 32U;
             vec_memcpy(local,
-                       tileB + cols * (__anf03 * 32U) + mcol * 32U +
+                       tileB + cols * (__anf06 * 32U) + mcol * 32U +
                        cols * row + col);
             uint32_t k = 0U;
             for (; k < 4U; k++)
@@ -2772,14 +2823,15 @@ __hoisted_25(float alpha,
     for (; resIdxM < 8U; resIdxM++) {
         uint32_t resIdxN = 0U;
         for (; resIdxN < 16U; resIdxN++)
-            t_tile[(blockIdx.x / (cols / 32U) * 64U + threadIdx.x / 2U * 8U +
-                    resIdxM) * cols + blockIdx.x % (cols / 32U) * 32U +
-                   threadIdx.x % 2U * 16U + resIdxN]
+            t_tile[(64U * (blockIdx.x / (cols / 32U)) +
+                    8U * (threadIdx.x / 2U) + resIdxM) * cols +
+                   32U * (blockIdx.x % (cols / 32U)) +
+                   16U * (threadIdx.x % 2U) + resIdxN]
                 = beta *
-                t_tile[(blockIdx.x / (cols / 32U) * 64U +
-                        threadIdx.x / 2U * 8U + resIdxM) * cols +
-                       blockIdx.x % (cols / 32U) * 32U +
-                       threadIdx.x % 2U * 16U + resIdxN]
+                t_tile[(64U * (blockIdx.x / (cols / 32U)) +
+                        8U * (threadIdx.x / 2U) + resIdxM) * cols +
+                       32U * (blockIdx.x % (cols / 32U)) +
+                       16U * (threadIdx.x % 2U) + resIdxN]
                 + alpha * rchProd[resIdxM * 16U + resIdxN];
     }
 }
@@ -2838,6 +2890,7 @@ __hoisted_26(float alpha,
             for (; k < 4U; k++)
                 sA[(col + k) * 64U + row] = local[k];
         }
+        uint32_t __anf06 = bkIdx;
         float *tileB = gB;
         uint32_t i = 0U;
         for (; i < 1024U; i += 64U) {
@@ -2846,7 +2899,7 @@ __hoisted_26(float alpha,
             uint32_t row = (i + threadIdx.x * 4U) / 32U;
             uint32_t col = (i + threadIdx.x * 4U) % 32U;
             vec_memcpy(local,
-                       tileB + cols * (__anf03 * 32U) + mcol * 32U +
+                       tileB + cols * (__anf06 * 32U) + mcol * 32U +
                        cols * row + col);
             uint32_t k = 0U;
             for (; k < 4U; k++)
@@ -2880,14 +2933,15 @@ __hoisted_26(float alpha,
     for (; resIdxM < 16U; resIdxM++) {
         uint32_t resIdxN = 0U;
         for (; resIdxN < 8U; resIdxN++)
-            t_tile[(blockIdx.x / (cols / 32U) * 64U + threadIdx.x / 4U * 16U +
-                    resIdxM) * cols + blockIdx.x % (cols / 32U) * 32U +
-                   threadIdx.x % 4U * 8U + resIdxN]
+            t_tile[(64U * (blockIdx.x / (cols / 32U)) +
+                    16U * (threadIdx.x / 4U) + resIdxM) * cols +
+                   32U * (blockIdx.x % (cols / 32U)) + 8U * (threadIdx.x % 4U) +
+                   resIdxN]
                 = beta *
-                t_tile[(blockIdx.x / (cols / 32U) * 64U +
-                        threadIdx.x / 4U * 16U + resIdxM) * cols +
-                       blockIdx.x % (cols / 32U) * 32U + threadIdx.x % 4U * 8U +
-                       resIdxN]
+                t_tile[(64U * (blockIdx.x / (cols / 32U)) +
+                        16U * (threadIdx.x / 4U) + resIdxM) * cols +
+                       32U * (blockIdx.x % (cols / 32U)) +
+                       8U * (threadIdx.x % 4U) + resIdxN]
                 + alpha * rchProd[resIdxM * 8U + resIdxN];
     }
 }
@@ -2946,6 +3000,7 @@ __hoisted_27(float alpha,
             for (; k < 4U; k++)
                 sA[(col + k) * 64U + row] = local[k];
         }
+        uint32_t __anf06 = bkIdx;
         float *tileB = gB;
         uint32_t i = 0U;
         for (; i < 1024U; i += 32U) {
@@ -2954,7 +3009,7 @@ __hoisted_27(float alpha,
             uint32_t row = (i + threadIdx.x * 4U) / 32U;
             uint32_t col = (i + threadIdx.x * 4U) % 32U;
             vec_memcpy(local,
-                       tileB + cols * (__anf03 * 32U) + mcol * 32U +
+                       tileB + cols * (__anf06 * 32U) + mcol * 32U +
                        cols * row + col);
             uint32_t k = 0U;
             for (; k < 4U; k++)
@@ -2988,14 +3043,15 @@ __hoisted_27(float alpha,
     for (; resIdxM < 16U; resIdxM++) {
         uint32_t resIdxN = 0U;
         for (; resIdxN < 16U; resIdxN++)
-            t_tile[(blockIdx.x / (cols / 32U) * 64U + threadIdx.x / 2U * 16U +
-                    resIdxM) * cols + blockIdx.x % (cols / 32U) * 32U +
-                   threadIdx.x % 2U * 16U + resIdxN]
+            t_tile[(64U * (blockIdx.x / (cols / 32U)) +
+                    16U * (threadIdx.x / 2U) + resIdxM) * cols +
+                   32U * (blockIdx.x % (cols / 32U)) +
+                   16U * (threadIdx.x % 2U) + resIdxN]
                 = beta *
-                t_tile[(blockIdx.x / (cols / 32U) * 64U +
-                        threadIdx.x / 2U * 16U + resIdxM) * cols +
-                       blockIdx.x % (cols / 32U) * 32U +
-                       threadIdx.x % 2U * 16U + resIdxN]
+                t_tile[(64U * (blockIdx.x / (cols / 32U)) +
+                        16U * (threadIdx.x / 2U) + resIdxM) * cols +
+                       32U * (blockIdx.x % (cols / 32U)) +
+                       16U * (threadIdx.x % 2U) + resIdxN]
                 + alpha * rchProd[resIdxM * 16U + resIdxN];
     }
 }
@@ -3054,6 +3110,7 @@ __hoisted_28(float alpha,
             for (; k < 4U; k++)
                 sA[(col + k) * 64U + row] = local[k];
         }
+        uint32_t __anf06 = bkIdx;
         float *tileB = gB;
         uint32_t i = 0U;
         for (; i < 2048U; i += 128U) {
@@ -3062,7 +3119,7 @@ __hoisted_28(float alpha,
             uint32_t row = (i + threadIdx.x * 4U) / 32U;
             uint32_t col = (i + threadIdx.x * 4U) % 32U;
             vec_memcpy(local,
-                       tileB + cols * (__anf03 * 64U) + mcol * 32U +
+                       tileB + cols * (__anf06 * 64U) + mcol * 32U +
                        cols * row + col);
             uint32_t k = 0U;
             for (; k < 4U; k++)
@@ -3096,14 +3153,15 @@ __hoisted_28(float alpha,
     for (; resIdxM < 8U; resIdxM++) {
         uint32_t resIdxN = 0U;
         for (; resIdxN < 8U; resIdxN++)
-            t_tile[(blockIdx.x / (cols / 32U) * 64U + threadIdx.x / 4U * 8U +
-                    resIdxM) * cols + blockIdx.x % (cols / 32U) * 32U +
-                   threadIdx.x % 4U * 8U + resIdxN]
+            t_tile[(64U * (blockIdx.x / (cols / 32U)) +
+                    8U * (threadIdx.x / 4U) + resIdxM) * cols +
+                   32U * (blockIdx.x % (cols / 32U)) + 8U * (threadIdx.x % 4U) +
+                   resIdxN]
                 = beta *
-                t_tile[(blockIdx.x / (cols / 32U) * 64U +
-                        threadIdx.x / 4U * 8U + resIdxM) * cols +
-                       blockIdx.x % (cols / 32U) * 32U + threadIdx.x % 4U * 8U +
-                       resIdxN]
+                t_tile[(64U * (blockIdx.x / (cols / 32U)) +
+                        8U * (threadIdx.x / 4U) + resIdxM) * cols +
+                       32U * (blockIdx.x % (cols / 32U)) +
+                       8U * (threadIdx.x % 4U) + resIdxN]
                 + alpha * rchProd[resIdxM * 8U + resIdxN];
     }
 }
@@ -3161,6 +3219,7 @@ __hoisted_29(float alpha,
             for (; k < 4U; k++)
                 sA[(col + k) * 64U + row] = local[k];
         }
+        uint32_t __anf06 = bkIdx;
         float *tileB = gB;
         uint32_t i = 0U;
         for (; i < 2048U; i += 64U) {
@@ -3169,7 +3228,7 @@ __hoisted_29(float alpha,
             uint32_t row = (i + threadIdx.x * 4U) / 32U;
             uint32_t col = (i + threadIdx.x * 4U) % 32U;
             vec_memcpy(local,
-                       tileB + cols * (__anf03 * 64U) + mcol * 32U +
+                       tileB + cols * (__anf06 * 64U) + mcol * 32U +
                        cols * row + col);
             uint32_t k = 0U;
             for (; k < 4U; k++)
@@ -3203,14 +3262,15 @@ __hoisted_29(float alpha,
     for (; resIdxM < 8U; resIdxM++) {
         uint32_t resIdxN = 0U;
         for (; resIdxN < 16U; resIdxN++)
-            t_tile[(blockIdx.x / (cols / 32U) * 64U + threadIdx.x / 2U * 8U +
-                    resIdxM) * cols + blockIdx.x % (cols / 32U) * 32U +
-                   threadIdx.x % 2U * 16U + resIdxN]
+            t_tile[(64U * (blockIdx.x / (cols / 32U)) +
+                    8U * (threadIdx.x / 2U) + resIdxM) * cols +
+                   32U * (blockIdx.x % (cols / 32U)) +
+                   16U * (threadIdx.x % 2U) + resIdxN]
                 = beta *
-                t_tile[(blockIdx.x / (cols / 32U) * 64U +
-                        threadIdx.x / 2U * 8U + resIdxM) * cols +
-                       blockIdx.x % (cols / 32U) * 32U +
-                       threadIdx.x % 2U * 16U + resIdxN]
+                t_tile[(64U * (blockIdx.x / (cols / 32U)) +
+                        8U * (threadIdx.x / 2U) + resIdxM) * cols +
+                       32U * (blockIdx.x % (cols / 32U)) +
+                       16U * (threadIdx.x % 2U) + resIdxN]
                 + alpha * rchProd[resIdxM * 16U + resIdxN];
     }
 }
@@ -3269,6 +3329,7 @@ __hoisted_30(float alpha,
             for (; k < 4U; k++)
                 sA[(col + k) * 64U + row] = local[k];
         }
+        uint32_t __anf06 = bkIdx;
         float *tileB = gB;
         uint32_t i = 0U;
         for (; i < 2048U; i += 64U) {
@@ -3277,7 +3338,7 @@ __hoisted_30(float alpha,
             uint32_t row = (i + threadIdx.x * 4U) / 32U;
             uint32_t col = (i + threadIdx.x * 4U) % 32U;
             vec_memcpy(local,
-                       tileB + cols * (__anf03 * 64U) + mcol * 32U +
+                       tileB + cols * (__anf06 * 64U) + mcol * 32U +
                        cols * row + col);
             uint32_t k = 0U;
             for (; k < 4U; k++)
@@ -3311,14 +3372,15 @@ __hoisted_30(float alpha,
     for (; resIdxM < 16U; resIdxM++) {
         uint32_t resIdxN = 0U;
         for (; resIdxN < 8U; resIdxN++)
-            t_tile[(blockIdx.x / (cols / 32U) * 64U + threadIdx.x / 4U * 16U +
-                    resIdxM) * cols + blockIdx.x % (cols / 32U) * 32U +
-                   threadIdx.x % 4U * 8U + resIdxN]
+            t_tile[(64U * (blockIdx.x / (cols / 32U)) +
+                    16U * (threadIdx.x / 4U) + resIdxM) * cols +
+                   32U * (blockIdx.x % (cols / 32U)) + 8U * (threadIdx.x % 4U) +
+                   resIdxN]
                 = beta *
-                t_tile[(blockIdx.x / (cols / 32U) * 64U +
-                        threadIdx.x / 4U * 16U + resIdxM) * cols +
-                       blockIdx.x % (cols / 32U) * 32U + threadIdx.x % 4U * 8U +
-                       resIdxN]
+                t_tile[(64U * (blockIdx.x / (cols / 32U)) +
+                        16U * (threadIdx.x / 4U) + resIdxM) * cols +
+                       32U * (blockIdx.x % (cols / 32U)) +
+                       8U * (threadIdx.x % 4U) + resIdxN]
                 + alpha * rchProd[resIdxM * 8U + resIdxN];
     }
 }
@@ -3377,6 +3439,7 @@ __hoisted_31(float alpha,
             for (; k < 4U; k++)
                 sA[(col + k) * 64U + row] = local[k];
         }
+        uint32_t __anf06 = bkIdx;
         float *tileB = gB;
         uint32_t i = 0U;
         for (; i < 2048U; i += 32U) {
@@ -3385,7 +3448,7 @@ __hoisted_31(float alpha,
             uint32_t row = (i + threadIdx.x * 4U) / 32U;
             uint32_t col = (i + threadIdx.x * 4U) % 32U;
             vec_memcpy(local,
-                       tileB + cols * (__anf03 * 64U) + mcol * 32U +
+                       tileB + cols * (__anf06 * 64U) + mcol * 32U +
                        cols * row + col);
             uint32_t k = 0U;
             for (; k < 4U; k++)
@@ -3419,14 +3482,15 @@ __hoisted_31(float alpha,
     for (; resIdxM < 16U; resIdxM++) {
         uint32_t resIdxN = 0U;
         for (; resIdxN < 16U; resIdxN++)
-            t_tile[(blockIdx.x / (cols / 32U) * 64U + threadIdx.x / 2U * 16U +
-                    resIdxM) * cols + blockIdx.x % (cols / 32U) * 32U +
-                   threadIdx.x % 2U * 16U + resIdxN]
+            t_tile[(64U * (blockIdx.x / (cols / 32U)) +
+                    16U * (threadIdx.x / 2U) + resIdxM) * cols +
+                   32U * (blockIdx.x % (cols / 32U)) +
+                   16U * (threadIdx.x % 2U) + resIdxN]
                 = beta *
-                t_tile[(blockIdx.x / (cols / 32U) * 64U +
-                        threadIdx.x / 2U * 16U + resIdxM) * cols +
-                       blockIdx.x % (cols / 32U) * 32U +
-                       threadIdx.x % 2U * 16U + resIdxN]
+                t_tile[(64U * (blockIdx.x / (cols / 32U)) +
+                        16U * (threadIdx.x / 2U) + resIdxM) * cols +
+                       32U * (blockIdx.x % (cols / 32U)) +
+                       16U * (threadIdx.x % 2U) + resIdxN]
                 + alpha * rchProd[resIdxM * 16U + resIdxN];
     }
 }
@@ -3485,6 +3549,7 @@ __hoisted_32(float alpha,
             for (; k < 4U; k++)
                 sA[(col + k) * 64U + row] = local[k];
         }
+        uint32_t __anf06 = bkIdx;
         float *tileB = gB;
         uint32_t i = 0U;
         for (; i < 2048U; i += 256U) {
@@ -3493,7 +3558,7 @@ __hoisted_32(float alpha,
             uint32_t row = (i + threadIdx.x * 4U) / 64U;
             uint32_t col = (i + threadIdx.x * 4U) % 64U;
             vec_memcpy(local,
-                       tileB + cols * (__anf03 * 32U) + mcol * 64U +
+                       tileB + cols * (__anf06 * 32U) + mcol * 64U +
                        cols * row + col);
             uint32_t k = 0U;
             for (; k < 4U; k++)
@@ -3527,14 +3592,15 @@ __hoisted_32(float alpha,
     for (; resIdxM < 8U; resIdxM++) {
         uint32_t resIdxN = 0U;
         for (; resIdxN < 8U; resIdxN++)
-            t_tile[(blockIdx.x / (cols / 64U) * 64U + threadIdx.x / 8U * 8U +
-                    resIdxM) * cols + blockIdx.x % (cols / 64U) * 64U +
-                   threadIdx.x % 8U * 8U + resIdxN]
+            t_tile[(64U * (blockIdx.x / (cols / 64U)) +
+                    8U * (threadIdx.x / 8U) + resIdxM) * cols +
+                   64U * (blockIdx.x % (cols / 64U)) + 8U * (threadIdx.x % 8U) +
+                   resIdxN]
                 = beta *
-                t_tile[(blockIdx.x / (cols / 64U) * 64U +
-                        threadIdx.x / 8U * 8U + resIdxM) * cols +
-                       blockIdx.x % (cols / 64U) * 64U + threadIdx.x % 8U * 8U +
-                       resIdxN]
+                t_tile[(64U * (blockIdx.x / (cols / 64U)) +
+                        8U * (threadIdx.x / 8U) + resIdxM) * cols +
+                       64U * (blockIdx.x % (cols / 64U)) +
+                       8U * (threadIdx.x % 8U) + resIdxN]
                 + alpha * rchProd[resIdxM * 8U + resIdxN];
     }
 }
@@ -3592,6 +3658,7 @@ __hoisted_33(float alpha,
             for (; k < 4U; k++)
                 sA[(col + k) * 64U + row] = local[k];
         }
+        uint32_t __anf06 = bkIdx;
         float *tileB = gB;
         uint32_t i = 0U;
         for (; i < 2048U; i += 128U) {
@@ -3600,7 +3667,7 @@ __hoisted_33(float alpha,
             uint32_t row = (i + threadIdx.x * 4U) / 64U;
             uint32_t col = (i + threadIdx.x * 4U) % 64U;
             vec_memcpy(local,
-                       tileB + cols * (__anf03 * 32U) + mcol * 64U +
+                       tileB + cols * (__anf06 * 32U) + mcol * 64U +
                        cols * row + col);
             uint32_t k = 0U;
             for (; k < 4U; k++)
@@ -3634,14 +3701,15 @@ __hoisted_33(float alpha,
     for (; resIdxM < 8U; resIdxM++) {
         uint32_t resIdxN = 0U;
         for (; resIdxN < 16U; resIdxN++)
-            t_tile[(blockIdx.x / (cols / 64U) * 64U + threadIdx.x / 4U * 8U +
-                    resIdxM) * cols + blockIdx.x % (cols / 64U) * 64U +
-                   threadIdx.x % 4U * 16U + resIdxN]
+            t_tile[(64U * (blockIdx.x / (cols / 64U)) +
+                    8U * (threadIdx.x / 4U) + resIdxM) * cols +
+                   64U * (blockIdx.x % (cols / 64U)) +
+                   16U * (threadIdx.x % 4U) + resIdxN]
                 = beta *
-                t_tile[(blockIdx.x / (cols / 64U) * 64U +
-                        threadIdx.x / 4U * 8U + resIdxM) * cols +
-                       blockIdx.x % (cols / 64U) * 64U +
-                       threadIdx.x % 4U * 16U + resIdxN]
+                t_tile[(64U * (blockIdx.x / (cols / 64U)) +
+                        8U * (threadIdx.x / 4U) + resIdxM) * cols +
+                       64U * (blockIdx.x % (cols / 64U)) +
+                       16U * (threadIdx.x % 4U) + resIdxN]
                 + alpha * rchProd[resIdxM * 16U + resIdxN];
     }
 }
@@ -3700,6 +3768,7 @@ __hoisted_34(float alpha,
             for (; k < 4U; k++)
                 sA[(col + k) * 64U + row] = local[k];
         }
+        uint32_t __anf06 = bkIdx;
         float *tileB = gB;
         uint32_t i = 0U;
         for (; i < 2048U; i += 128U) {
@@ -3708,7 +3777,7 @@ __hoisted_34(float alpha,
             uint32_t row = (i + threadIdx.x * 4U) / 64U;
             uint32_t col = (i + threadIdx.x * 4U) % 64U;
             vec_memcpy(local,
-                       tileB + cols * (__anf03 * 32U) + mcol * 64U +
+                       tileB + cols * (__anf06 * 32U) + mcol * 64U +
                        cols * row + col);
             uint32_t k = 0U;
             for (; k < 4U; k++)
@@ -3742,14 +3811,15 @@ __hoisted_34(float alpha,
     for (; resIdxM < 16U; resIdxM++) {
         uint32_t resIdxN = 0U;
         for (; resIdxN < 8U; resIdxN++)
-            t_tile[(blockIdx.x / (cols / 64U) * 64U + threadIdx.x / 8U * 16U +
-                    resIdxM) * cols + blockIdx.x % (cols / 64U) * 64U +
-                   threadIdx.x % 8U * 8U + resIdxN]
+            t_tile[(64U * (blockIdx.x / (cols / 64U)) +
+                    16U * (threadIdx.x / 8U) + resIdxM) * cols +
+                   64U * (blockIdx.x % (cols / 64U)) + 8U * (threadIdx.x % 8U) +
+                   resIdxN]
                 = beta *
-                t_tile[(blockIdx.x / (cols / 64U) * 64U +
-                        threadIdx.x / 8U * 16U + resIdxM) * cols +
-                       blockIdx.x % (cols / 64U) * 64U + threadIdx.x % 8U * 8U +
-                       resIdxN]
+                t_tile[(64U * (blockIdx.x / (cols / 64U)) +
+                        16U * (threadIdx.x / 8U) + resIdxM) * cols +
+                       64U * (blockIdx.x % (cols / 64U)) +
+                       8U * (threadIdx.x % 8U) + resIdxN]
                 + alpha * rchProd[resIdxM * 8U + resIdxN];
     }
 }
@@ -3808,6 +3878,7 @@ __hoisted_35(float alpha,
             for (; k < 4U; k++)
                 sA[(col + k) * 64U + row] = local[k];
         }
+        uint32_t __anf06 = bkIdx;
         float *tileB = gB;
         uint32_t i = 0U;
         for (; i < 2048U; i += 64U) {
@@ -3816,7 +3887,7 @@ __hoisted_35(float alpha,
             uint32_t row = (i + threadIdx.x * 4U) / 64U;
             uint32_t col = (i + threadIdx.x * 4U) % 64U;
             vec_memcpy(local,
-                       tileB + cols * (__anf03 * 32U) + mcol * 64U +
+                       tileB + cols * (__anf06 * 32U) + mcol * 64U +
                        cols * row + col);
             uint32_t k = 0U;
             for (; k < 4U; k++)
@@ -3850,14 +3921,15 @@ __hoisted_35(float alpha,
     for (; resIdxM < 16U; resIdxM++) {
         uint32_t resIdxN = 0U;
         for (; resIdxN < 16U; resIdxN++)
-            t_tile[(blockIdx.x / (cols / 64U) * 64U + threadIdx.x / 4U * 16U +
-                    resIdxM) * cols + blockIdx.x % (cols / 64U) * 64U +
-                   threadIdx.x % 4U * 16U + resIdxN]
+            t_tile[(64U * (blockIdx.x / (cols / 64U)) +
+                    16U * (threadIdx.x / 4U) + resIdxM) * cols +
+                   64U * (blockIdx.x % (cols / 64U)) +
+                   16U * (threadIdx.x % 4U) + resIdxN]
                 = beta *
-                t_tile[(blockIdx.x / (cols / 64U) * 64U +
-                        threadIdx.x / 4U * 16U + resIdxM) * cols +
-                       blockIdx.x % (cols / 64U) * 64U +
-                       threadIdx.x % 4U * 16U + resIdxN]
+                t_tile[(64U * (blockIdx.x / (cols / 64U)) +
+                        16U * (threadIdx.x / 4U) + resIdxM) * cols +
+                       64U * (blockIdx.x % (cols / 64U)) +
+                       16U * (threadIdx.x % 4U) + resIdxN]
                 + alpha * rchProd[resIdxM * 16U + resIdxN];
     }
 }
@@ -3916,6 +3988,7 @@ __hoisted_36(float alpha,
             for (; k < 4U; k++)
                 sA[(col + k) * 64U + row] = local[k];
         }
+        uint32_t __anf06 = bkIdx;
         float *tileB = gB;
         uint32_t i = 0U;
         for (; i < 4096U; i += 256U) {
@@ -3924,7 +3997,7 @@ __hoisted_36(float alpha,
             uint32_t row = (i + threadIdx.x * 4U) / 64U;
             uint32_t col = (i + threadIdx.x * 4U) % 64U;
             vec_memcpy(local,
-                       tileB + cols * (__anf03 * 64U) + mcol * 64U +
+                       tileB + cols * (__anf06 * 64U) + mcol * 64U +
                        cols * row + col);
             uint32_t k = 0U;
             for (; k < 4U; k++)
@@ -3958,14 +4031,15 @@ __hoisted_36(float alpha,
     for (; resIdxM < 8U; resIdxM++) {
         uint32_t resIdxN = 0U;
         for (; resIdxN < 8U; resIdxN++)
-            t_tile[(blockIdx.x / (cols / 64U) * 64U + threadIdx.x / 8U * 8U +
-                    resIdxM) * cols + blockIdx.x % (cols / 64U) * 64U +
-                   threadIdx.x % 8U * 8U + resIdxN]
+            t_tile[(64U * (blockIdx.x / (cols / 64U)) +
+                    8U * (threadIdx.x / 8U) + resIdxM) * cols +
+                   64U * (blockIdx.x % (cols / 64U)) + 8U * (threadIdx.x % 8U) +
+                   resIdxN]
                 = beta *
-                t_tile[(blockIdx.x / (cols / 64U) * 64U +
-                        threadIdx.x / 8U * 8U + resIdxM) * cols +
-                       blockIdx.x % (cols / 64U) * 64U + threadIdx.x % 8U * 8U +
-                       resIdxN]
+                t_tile[(64U * (blockIdx.x / (cols / 64U)) +
+                        8U * (threadIdx.x / 8U) + resIdxM) * cols +
+                       64U * (blockIdx.x % (cols / 64U)) +
+                       8U * (threadIdx.x % 8U) + resIdxN]
                 + alpha * rchProd[resIdxM * 8U + resIdxN];
     }
 }
@@ -4023,6 +4097,7 @@ __hoisted_37(float alpha,
             for (; k < 4U; k++)
                 sA[(col + k) * 64U + row] = local[k];
         }
+        uint32_t __anf06 = bkIdx;
         float *tileB = gB;
         uint32_t i = 0U;
         for (; i < 4096U; i += 128U) {
@@ -4031,7 +4106,7 @@ __hoisted_37(float alpha,
             uint32_t row = (i + threadIdx.x * 4U) / 64U;
             uint32_t col = (i + threadIdx.x * 4U) % 64U;
             vec_memcpy(local,
-                       tileB + cols * (__anf03 * 64U) + mcol * 64U +
+                       tileB + cols * (__anf06 * 64U) + mcol * 64U +
                        cols * row + col);
             uint32_t k = 0U;
             for (; k < 4U; k++)
@@ -4065,14 +4140,15 @@ __hoisted_37(float alpha,
     for (; resIdxM < 8U; resIdxM++) {
         uint32_t resIdxN = 0U;
         for (; resIdxN < 16U; resIdxN++)
-            t_tile[(blockIdx.x / (cols / 64U) * 64U + threadIdx.x / 4U * 8U +
-                    resIdxM) * cols + blockIdx.x % (cols / 64U) * 64U +
-                   threadIdx.x % 4U * 16U + resIdxN]
+            t_tile[(64U * (blockIdx.x / (cols / 64U)) +
+                    8U * (threadIdx.x / 4U) + resIdxM) * cols +
+                   64U * (blockIdx.x % (cols / 64U)) +
+                   16U * (threadIdx.x % 4U) + resIdxN]
                 = beta *
-                t_tile[(blockIdx.x / (cols / 64U) * 64U +
-                        threadIdx.x / 4U * 8U + resIdxM) * cols +
-                       blockIdx.x % (cols / 64U) * 64U +
-                       threadIdx.x % 4U * 16U + resIdxN]
+                t_tile[(64U * (blockIdx.x / (cols / 64U)) +
+                        8U * (threadIdx.x / 4U) + resIdxM) * cols +
+                       64U * (blockIdx.x % (cols / 64U)) +
+                       16U * (threadIdx.x % 4U) + resIdxN]
                 + alpha * rchProd[resIdxM * 16U + resIdxN];
     }
 }
@@ -4131,6 +4207,7 @@ __hoisted_38(float alpha,
             for (; k < 4U; k++)
                 sA[(col + k) * 64U + row] = local[k];
         }
+        uint32_t __anf06 = bkIdx;
         float *tileB = gB;
         uint32_t i = 0U;
         for (; i < 4096U; i += 128U) {
@@ -4139,7 +4216,7 @@ __hoisted_38(float alpha,
             uint32_t row = (i + threadIdx.x * 4U) / 64U;
             uint32_t col = (i + threadIdx.x * 4U) % 64U;
             vec_memcpy(local,
-                       tileB + cols * (__anf03 * 64U) + mcol * 64U +
+                       tileB + cols * (__anf06 * 64U) + mcol * 64U +
                        cols * row + col);
             uint32_t k = 0U;
             for (; k < 4U; k++)
@@ -4173,14 +4250,15 @@ __hoisted_38(float alpha,
     for (; resIdxM < 16U; resIdxM++) {
         uint32_t resIdxN = 0U;
         for (; resIdxN < 8U; resIdxN++)
-            t_tile[(blockIdx.x / (cols / 64U) * 64U + threadIdx.x / 8U * 16U +
-                    resIdxM) * cols + blockIdx.x % (cols / 64U) * 64U +
-                   threadIdx.x % 8U * 8U + resIdxN]
+            t_tile[(64U * (blockIdx.x / (cols / 64U)) +
+                    16U * (threadIdx.x / 8U) + resIdxM) * cols +
+                   64U * (blockIdx.x % (cols / 64U)) + 8U * (threadIdx.x % 8U) +
+                   resIdxN]
                 = beta *
-                t_tile[(blockIdx.x / (cols / 64U) * 64U +
-                        threadIdx.x / 8U * 16U + resIdxM) * cols +
-                       blockIdx.x % (cols / 64U) * 64U + threadIdx.x % 8U * 8U +
-                       resIdxN]
+                t_tile[(64U * (blockIdx.x / (cols / 64U)) +
+                        16U * (threadIdx.x / 8U) + resIdxM) * cols +
+                       64U * (blockIdx.x % (cols / 64U)) +
+                       8U * (threadIdx.x % 8U) + resIdxN]
                 + alpha * rchProd[resIdxM * 8U + resIdxN];
     }
 }
@@ -4239,6 +4317,7 @@ __hoisted_39(float alpha,
             for (; k < 4U; k++)
                 sA[(col + k) * 64U + row] = local[k];
         }
+        uint32_t __anf06 = bkIdx;
         float *tileB = gB;
         uint32_t i = 0U;
         for (; i < 4096U; i += 64U) {
@@ -4247,7 +4326,7 @@ __hoisted_39(float alpha,
             uint32_t row = (i + threadIdx.x * 4U) / 64U;
             uint32_t col = (i + threadIdx.x * 4U) % 64U;
             vec_memcpy(local,
-                       tileB + cols * (__anf03 * 64U) + mcol * 64U +
+                       tileB + cols * (__anf06 * 64U) + mcol * 64U +
                        cols * row + col);
             uint32_t k = 0U;
             for (; k < 4U; k++)
@@ -4281,14 +4360,15 @@ __hoisted_39(float alpha,
     for (; resIdxM < 16U; resIdxM++) {
         uint32_t resIdxN = 0U;
         for (; resIdxN < 16U; resIdxN++)
-            t_tile[(blockIdx.x / (cols / 64U) * 64U + threadIdx.x / 4U * 16U +
-                    resIdxM) * cols + blockIdx.x % (cols / 64U) * 64U +
-                   threadIdx.x % 4U * 16U + resIdxN]
+            t_tile[(64U * (blockIdx.x / (cols / 64U)) +
+                    16U * (threadIdx.x / 4U) + resIdxM) * cols +
+                   64U * (blockIdx.x % (cols / 64U)) +
+                   16U * (threadIdx.x % 4U) + resIdxN]
                 = beta *
-                t_tile[(blockIdx.x / (cols / 64U) * 64U +
-                        threadIdx.x / 4U * 16U + resIdxM) * cols +
-                       blockIdx.x % (cols / 64U) * 64U +
-                       threadIdx.x % 4U * 16U + resIdxN]
+                t_tile[(64U * (blockIdx.x / (cols / 64U)) +
+                        16U * (threadIdx.x / 4U) + resIdxM) * cols +
+                       64U * (blockIdx.x % (cols / 64U)) +
+                       16U * (threadIdx.x % 4U) + resIdxN]
                 + alpha * rchProd[resIdxM * 16U + resIdxN];
     }
 }
@@ -4347,6 +4427,7 @@ __hoisted_40(float alpha,
             for (; k < 4U; k++)
                 sA[(col + k) * 64U + row] = local[k];
         }
+        uint32_t __anf06 = bkIdx;
         float *tileB = gB;
         uint32_t i = 0U;
         for (; i < 4096U; i += 512U) {
@@ -4355,7 +4436,7 @@ __hoisted_40(float alpha,
             uint32_t row = (i + threadIdx.x * 4U) / 128U;
             uint32_t col = (i + threadIdx.x * 4U) % 128U;
             vec_memcpy(local,
-                       tileB + cols * (__anf03 * 32U) + mcol * 128U +
+                       tileB + cols * (__anf06 * 32U) + mcol * 128U +
                        cols * row + col);
             uint32_t k = 0U;
             for (; k < 4U; k++)
@@ -4389,14 +4470,15 @@ __hoisted_40(float alpha,
     for (; resIdxM < 8U; resIdxM++) {
         uint32_t resIdxN = 0U;
         for (; resIdxN < 8U; resIdxN++)
-            t_tile[(blockIdx.x / (cols / 128U) * 64U + threadIdx.x / 16U * 8U +
-                    resIdxM) * cols + blockIdx.x % (cols / 128U) * 128U +
-                   threadIdx.x % 16U * 8U + resIdxN]
+            t_tile[(64U * (blockIdx.x / (cols / 128U)) +
+                    8U * (threadIdx.x / 16U) + resIdxM) * cols +
+                   128U * (blockIdx.x % (cols / 128U)) +
+                   8U * (threadIdx.x % 16U) + resIdxN]
                 = beta *
-                t_tile[(blockIdx.x / (cols / 128U) * 64U +
-                        threadIdx.x / 16U * 8U + resIdxM) * cols +
-                       blockIdx.x % (cols / 128U) * 128U +
-                       threadIdx.x % 16U * 8U + resIdxN]
+                t_tile[(64U * (blockIdx.x / (cols / 128U)) +
+                        8U * (threadIdx.x / 16U) + resIdxM) * cols +
+                       128U * (blockIdx.x % (cols / 128U)) +
+                       8U * (threadIdx.x % 16U) + resIdxN]
                 + alpha * rchProd[resIdxM * 8U + resIdxN];
     }
 }
@@ -4455,6 +4537,7 @@ __hoisted_41(float alpha,
             for (; k < 4U; k++)
                 sA[(col + k) * 64U + row] = local[k];
         }
+        uint32_t __anf06 = bkIdx;
         float *tileB = gB;
         uint32_t i = 0U;
         for (; i < 4096U; i += 256U) {
@@ -4463,7 +4546,7 @@ __hoisted_41(float alpha,
             uint32_t row = (i + threadIdx.x * 4U) / 128U;
             uint32_t col = (i + threadIdx.x * 4U) % 128U;
             vec_memcpy(local,
-                       tileB + cols * (__anf03 * 32U) + mcol * 128U +
+                       tileB + cols * (__anf06 * 32U) + mcol * 128U +
                        cols * row + col);
             uint32_t k = 0U;
             for (; k < 4U; k++)
@@ -4497,14 +4580,15 @@ __hoisted_41(float alpha,
     for (; resIdxM < 8U; resIdxM++) {
         uint32_t resIdxN = 0U;
         for (; resIdxN < 16U; resIdxN++)
-            t_tile[(blockIdx.x / (cols / 128U) * 64U + threadIdx.x / 8U * 8U +
-                    resIdxM) * cols + blockIdx.x % (cols / 128U) * 128U +
-                   threadIdx.x % 8U * 16U + resIdxN]
+            t_tile[(64U * (blockIdx.x / (cols / 128U)) +
+                    8U * (threadIdx.x / 8U) + resIdxM) * cols +
+                   128U * (blockIdx.x % (cols / 128U)) +
+                   16U * (threadIdx.x % 8U) + resIdxN]
                 = beta *
-                t_tile[(blockIdx.x / (cols / 128U) * 64U +
-                        threadIdx.x / 8U * 8U + resIdxM) * cols +
-                       blockIdx.x % (cols / 128U) * 128U +
-                       threadIdx.x % 8U * 16U + resIdxN]
+                t_tile[(64U * (blockIdx.x / (cols / 128U)) +
+                        8U * (threadIdx.x / 8U) + resIdxM) * cols +
+                       128U * (blockIdx.x % (cols / 128U)) +
+                       16U * (threadIdx.x % 8U) + resIdxN]
                 + alpha * rchProd[resIdxM * 16U + resIdxN];
     }
 }
@@ -4563,6 +4647,7 @@ __hoisted_42(float alpha,
             for (; k < 4U; k++)
                 sA[(col + k) * 64U + row] = local[k];
         }
+        uint32_t __anf06 = bkIdx;
         float *tileB = gB;
         uint32_t i = 0U;
         for (; i < 4096U; i += 256U) {
@@ -4571,7 +4656,7 @@ __hoisted_42(float alpha,
             uint32_t row = (i + threadIdx.x * 4U) / 128U;
             uint32_t col = (i + threadIdx.x * 4U) % 128U;
             vec_memcpy(local,
-                       tileB + cols * (__anf03 * 32U) + mcol * 128U +
+                       tileB + cols * (__anf06 * 32U) + mcol * 128U +
                        cols * row + col);
             uint32_t k = 0U;
             for (; k < 4U; k++)
@@ -4605,14 +4690,15 @@ __hoisted_42(float alpha,
     for (; resIdxM < 16U; resIdxM++) {
         uint32_t resIdxN = 0U;
         for (; resIdxN < 8U; resIdxN++)
-            t_tile[(blockIdx.x / (cols / 128U) * 64U + threadIdx.x / 16U * 16U +
-                    resIdxM) * cols + blockIdx.x % (cols / 128U) * 128U +
-                   threadIdx.x % 16U * 8U + resIdxN]
+            t_tile[(64U * (blockIdx.x / (cols / 128U)) +
+                    16U * (threadIdx.x / 16U) + resIdxM) * cols +
+                   128U * (blockIdx.x % (cols / 128U)) +
+                   8U * (threadIdx.x % 16U) + resIdxN]
                 = beta *
-                t_tile[(blockIdx.x / (cols / 128U) * 64U +
-                        threadIdx.x / 16U * 16U + resIdxM) * cols +
-                       blockIdx.x % (cols / 128U) * 128U +
-                       threadIdx.x % 16U * 8U + resIdxN]
+                t_tile[(64U * (blockIdx.x / (cols / 128U)) +
+                        16U * (threadIdx.x / 16U) + resIdxM) * cols +
+                       128U * (blockIdx.x % (cols / 128U)) +
+                       8U * (threadIdx.x % 16U) + resIdxN]
                 + alpha * rchProd[resIdxM * 8U + resIdxN];
     }
 }
@@ -4671,6 +4757,7 @@ __hoisted_43(float alpha,
             for (; k < 4U; k++)
                 sA[(col + k) * 64U + row] = local[k];
         }
+        uint32_t __anf06 = bkIdx;
         float *tileB = gB;
         uint32_t i = 0U;
         for (; i < 4096U; i += 128U) {
@@ -4679,7 +4766,7 @@ __hoisted_43(float alpha,
             uint32_t row = (i + threadIdx.x * 4U) / 128U;
             uint32_t col = (i + threadIdx.x * 4U) % 128U;
             vec_memcpy(local,
-                       tileB + cols * (__anf03 * 32U) + mcol * 128U +
+                       tileB + cols * (__anf06 * 32U) + mcol * 128U +
                        cols * row + col);
             uint32_t k = 0U;
             for (; k < 4U; k++)
@@ -4713,14 +4800,15 @@ __hoisted_43(float alpha,
     for (; resIdxM < 16U; resIdxM++) {
         uint32_t resIdxN = 0U;
         for (; resIdxN < 16U; resIdxN++)
-            t_tile[(blockIdx.x / (cols / 128U) * 64U + threadIdx.x / 8U * 16U +
-                    resIdxM) * cols + blockIdx.x % (cols / 128U) * 128U +
-                   threadIdx.x % 8U * 16U + resIdxN]
+            t_tile[(64U * (blockIdx.x / (cols / 128U)) +
+                    16U * (threadIdx.x / 8U) + resIdxM) * cols +
+                   128U * (blockIdx.x % (cols / 128U)) +
+                   16U * (threadIdx.x % 8U) + resIdxN]
                 = beta *
-                t_tile[(blockIdx.x / (cols / 128U) * 64U +
-                        threadIdx.x / 8U * 16U + resIdxM) * cols +
-                       blockIdx.x % (cols / 128U) * 128U +
-                       threadIdx.x % 8U * 16U + resIdxN]
+                t_tile[(64U * (blockIdx.x / (cols / 128U)) +
+                        16U * (threadIdx.x / 8U) + resIdxM) * cols +
+                       128U * (blockIdx.x % (cols / 128U)) +
+                       16U * (threadIdx.x % 8U) + resIdxN]
                 + alpha * rchProd[resIdxM * 16U + resIdxN];
     }
 }
@@ -4779,6 +4867,7 @@ __hoisted_44(float alpha,
             for (; k < 4U; k++)
                 sA[(col + k) * 64U + row] = local[k];
         }
+        uint32_t __anf06 = bkIdx;
         float *tileB = gB;
         uint32_t i = 0U;
         for (; i < 8192U; i += 512U) {
@@ -4787,7 +4876,7 @@ __hoisted_44(float alpha,
             uint32_t row = (i + threadIdx.x * 4U) / 128U;
             uint32_t col = (i + threadIdx.x * 4U) % 128U;
             vec_memcpy(local,
-                       tileB + cols * (__anf03 * 64U) + mcol * 128U +
+                       tileB + cols * (__anf06 * 64U) + mcol * 128U +
                        cols * row + col);
             uint32_t k = 0U;
             for (; k < 4U; k++)
@@ -4821,14 +4910,15 @@ __hoisted_44(float alpha,
     for (; resIdxM < 8U; resIdxM++) {
         uint32_t resIdxN = 0U;
         for (; resIdxN < 8U; resIdxN++)
-            t_tile[(blockIdx.x / (cols / 128U) * 64U + threadIdx.x / 16U * 8U +
-                    resIdxM) * cols + blockIdx.x % (cols / 128U) * 128U +
-                   threadIdx.x % 16U * 8U + resIdxN]
+            t_tile[(64U * (blockIdx.x / (cols / 128U)) +
+                    8U * (threadIdx.x / 16U) + resIdxM) * cols +
+                   128U * (blockIdx.x % (cols / 128U)) +
+                   8U * (threadIdx.x % 16U) + resIdxN]
                 = beta *
-                t_tile[(blockIdx.x / (cols / 128U) * 64U +
-                        threadIdx.x / 16U * 8U + resIdxM) * cols +
-                       blockIdx.x % (cols / 128U) * 128U +
-                       threadIdx.x % 16U * 8U + resIdxN]
+                t_tile[(64U * (blockIdx.x / (cols / 128U)) +
+                        8U * (threadIdx.x / 16U) + resIdxM) * cols +
+                       128U * (blockIdx.x % (cols / 128U)) +
+                       8U * (threadIdx.x % 16U) + resIdxN]
                 + alpha * rchProd[resIdxM * 8U + resIdxN];
     }
 }
@@ -4887,6 +4977,7 @@ __hoisted_45(float alpha,
             for (; k < 4U; k++)
                 sA[(col + k) * 64U + row] = local[k];
         }
+        uint32_t __anf06 = bkIdx;
         float *tileB = gB;
         uint32_t i = 0U;
         for (; i < 8192U; i += 256U) {
@@ -4895,7 +4986,7 @@ __hoisted_45(float alpha,
             uint32_t row = (i + threadIdx.x * 4U) / 128U;
             uint32_t col = (i + threadIdx.x * 4U) % 128U;
             vec_memcpy(local,
-                       tileB + cols * (__anf03 * 64U) + mcol * 128U +
+                       tileB + cols * (__anf06 * 64U) + mcol * 128U +
                        cols * row + col);
             uint32_t k = 0U;
             for (; k < 4U; k++)
@@ -4929,14 +5020,15 @@ __hoisted_45(float alpha,
     for (; resIdxM < 8U; resIdxM++) {
         uint32_t resIdxN = 0U;
         for (; resIdxN < 16U; resIdxN++)
-            t_tile[(blockIdx.x / (cols / 128U) * 64U + threadIdx.x / 8U * 8U +
-                    resIdxM) * cols + blockIdx.x % (cols / 128U) * 128U +
-                   threadIdx.x % 8U * 16U + resIdxN]
+            t_tile[(64U * (blockIdx.x / (cols / 128U)) +
+                    8U * (threadIdx.x / 8U) + resIdxM) * cols +
+                   128U * (blockIdx.x % (cols / 128U)) +
+                   16U * (threadIdx.x % 8U) + resIdxN]
                 = beta *
-                t_tile[(blockIdx.x / (cols / 128U) * 64U +
-                        threadIdx.x / 8U * 8U + resIdxM) * cols +
-                       blockIdx.x % (cols / 128U) * 128U +
-                       threadIdx.x % 8U * 16U + resIdxN]
+                t_tile[(64U * (blockIdx.x / (cols / 128U)) +
+                        8U * (threadIdx.x / 8U) + resIdxM) * cols +
+                       128U * (blockIdx.x % (cols / 128U)) +
+                       16U * (threadIdx.x % 8U) + resIdxN]
                 + alpha * rchProd[resIdxM * 16U + resIdxN];
     }
 }
@@ -4995,6 +5087,7 @@ __hoisted_46(float alpha,
             for (; k < 4U; k++)
                 sA[(col + k) * 64U + row] = local[k];
         }
+        uint32_t __anf06 = bkIdx;
         float *tileB = gB;
         uint32_t i = 0U;
         for (; i < 8192U; i += 256U) {
@@ -5003,7 +5096,7 @@ __hoisted_46(float alpha,
             uint32_t row = (i + threadIdx.x * 4U) / 128U;
             uint32_t col = (i + threadIdx.x * 4U) % 128U;
             vec_memcpy(local,
-                       tileB + cols * (__anf03 * 64U) + mcol * 128U +
+                       tileB + cols * (__anf06 * 64U) + mcol * 128U +
                        cols * row + col);
             uint32_t k = 0U;
             for (; k < 4U; k++)
@@ -5037,14 +5130,15 @@ __hoisted_46(float alpha,
     for (; resIdxM < 16U; resIdxM++) {
         uint32_t resIdxN = 0U;
         for (; resIdxN < 8U; resIdxN++)
-            t_tile[(blockIdx.x / (cols / 128U) * 64U + threadIdx.x / 16U * 16U +
-                    resIdxM) * cols + blockIdx.x % (cols / 128U) * 128U +
-                   threadIdx.x % 16U * 8U + resIdxN]
+            t_tile[(64U * (blockIdx.x / (cols / 128U)) +
+                    16U * (threadIdx.x / 16U) + resIdxM) * cols +
+                   128U * (blockIdx.x % (cols / 128U)) +
+                   8U * (threadIdx.x % 16U) + resIdxN]
                 = beta *
-                t_tile[(blockIdx.x / (cols / 128U) * 64U +
-                        threadIdx.x / 16U * 16U + resIdxM) * cols +
-                       blockIdx.x % (cols / 128U) * 128U +
-                       threadIdx.x % 16U * 8U + resIdxN]
+                t_tile[(64U * (blockIdx.x / (cols / 128U)) +
+                        16U * (threadIdx.x / 16U) + resIdxM) * cols +
+                       128U * (blockIdx.x % (cols / 128U)) +
+                       8U * (threadIdx.x % 16U) + resIdxN]
                 + alpha * rchProd[resIdxM * 8U + resIdxN];
     }
 }
@@ -5103,6 +5197,7 @@ __hoisted_47(float alpha,
             for (; k < 4U; k++)
                 sA[(col + k) * 64U + row] = local[k];
         }
+        uint32_t __anf06 = bkIdx;
         float *tileB = gB;
         uint32_t i = 0U;
         for (; i < 8192U; i += 128U) {
@@ -5111,7 +5206,7 @@ __hoisted_47(float alpha,
             uint32_t row = (i + threadIdx.x * 4U) / 128U;
             uint32_t col = (i + threadIdx.x * 4U) % 128U;
             vec_memcpy(local,
-                       tileB + cols * (__anf03 * 64U) + mcol * 128U +
+                       tileB + cols * (__anf06 * 64U) + mcol * 128U +
                        cols * row + col);
             uint32_t k = 0U;
             for (; k < 4U; k++)
@@ -5145,14 +5240,15 @@ __hoisted_47(float alpha,
     for (; resIdxM < 16U; resIdxM++) {
         uint32_t resIdxN = 0U;
         for (; resIdxN < 16U; resIdxN++)
-            t_tile[(blockIdx.x / (cols / 128U) * 64U + threadIdx.x / 8U * 16U +
-                    resIdxM) * cols + blockIdx.x % (cols / 128U) * 128U +
-                   threadIdx.x % 8U * 16U + resIdxN]
+            t_tile[(64U * (blockIdx.x / (cols / 128U)) +
+                    16U * (threadIdx.x / 8U) + resIdxM) * cols +
+                   128U * (blockIdx.x % (cols / 128U)) +
+                   16U * (threadIdx.x % 8U) + resIdxN]
                 = beta *
-                t_tile[(blockIdx.x / (cols / 128U) * 64U +
-                        threadIdx.x / 8U * 16U + resIdxM) * cols +
-                       blockIdx.x % (cols / 128U) * 128U +
-                       threadIdx.x % 8U * 16U + resIdxN]
+                t_tile[(64U * (blockIdx.x / (cols / 128U)) +
+                        16U * (threadIdx.x / 8U) + resIdxM) * cols +
+                       128U * (blockIdx.x % (cols / 128U)) +
+                       16U * (threadIdx.x % 8U) + resIdxN]
                 + alpha * rchProd[resIdxM * 16U + resIdxN];
     }
 }
@@ -5211,6 +5307,7 @@ __hoisted_48(float alpha,
             for (; k < 4U; k++)
                 sA[(col + k) * 128U + row] = local[k];
         }
+        uint32_t __anf06 = bkIdx;
         float *tileB = gB;
         uint32_t i = 0U;
         for (; i < 1024U; i += 256U) {
@@ -5219,7 +5316,7 @@ __hoisted_48(float alpha,
             uint32_t row = (i + threadIdx.x * 4U) / 32U;
             uint32_t col = (i + threadIdx.x * 4U) % 32U;
             vec_memcpy(local,
-                       tileB + cols * (__anf03 * 32U) + mcol * 32U +
+                       tileB + cols * (__anf06 * 32U) + mcol * 32U +
                        cols * row + col);
             uint32_t k = 0U;
             for (; k < 4U; k++)
@@ -5253,14 +5350,15 @@ __hoisted_48(float alpha,
     for (; resIdxM < 8U; resIdxM++) {
         uint32_t resIdxN = 0U;
         for (; resIdxN < 8U; resIdxN++)
-            t_tile[(blockIdx.x / (cols / 32U) * 128U + threadIdx.x / 4U * 8U +
-                    resIdxM) * cols + blockIdx.x % (cols / 32U) * 32U +
-                   threadIdx.x % 4U * 8U + resIdxN]
+            t_tile[(128U * (blockIdx.x / (cols / 32U)) +
+                    8U * (threadIdx.x / 4U) + resIdxM) * cols +
+                   32U * (blockIdx.x % (cols / 32U)) + 8U * (threadIdx.x % 4U) +
+                   resIdxN]
                 = beta *
-                t_tile[(blockIdx.x / (cols / 32U) * 128U +
-                        threadIdx.x / 4U * 8U + resIdxM) * cols +
-                       blockIdx.x % (cols / 32U) * 32U + threadIdx.x % 4U * 8U +
-                       resIdxN]
+                t_tile[(128U * (blockIdx.x / (cols / 32U)) +
+                        8U * (threadIdx.x / 4U) + resIdxM) * cols +
+                       32U * (blockIdx.x % (cols / 32U)) +
+                       8U * (threadIdx.x % 4U) + resIdxN]
                 + alpha * rchProd[resIdxM * 8U + resIdxN];
     }
 }
@@ -5319,6 +5417,7 @@ __hoisted_49(float alpha,
             for (; k < 4U; k++)
                 sA[(col + k) * 128U + row] = local[k];
         }
+        uint32_t __anf06 = bkIdx;
         float *tileB = gB;
         uint32_t i = 0U;
         for (; i < 1024U; i += 128U) {
@@ -5327,7 +5426,7 @@ __hoisted_49(float alpha,
             uint32_t row = (i + threadIdx.x * 4U) / 32U;
             uint32_t col = (i + threadIdx.x * 4U) % 32U;
             vec_memcpy(local,
-                       tileB + cols * (__anf03 * 32U) + mcol * 32U +
+                       tileB + cols * (__anf06 * 32U) + mcol * 32U +
                        cols * row + col);
             uint32_t k = 0U;
             for (; k < 4U; k++)
@@ -5361,14 +5460,15 @@ __hoisted_49(float alpha,
     for (; resIdxM < 8U; resIdxM++) {
         uint32_t resIdxN = 0U;
         for (; resIdxN < 16U; resIdxN++)
-            t_tile[(blockIdx.x / (cols / 32U) * 128U + threadIdx.x / 2U * 8U +
-                    resIdxM) * cols + blockIdx.x % (cols / 32U) * 32U +
-                   threadIdx.x % 2U * 16U + resIdxN]
+            t_tile[(128U * (blockIdx.x / (cols / 32U)) +
+                    8U * (threadIdx.x / 2U) + resIdxM) * cols +
+                   32U * (blockIdx.x % (cols / 32U)) +
+                   16U * (threadIdx.x % 2U) + resIdxN]
                 = beta *
-                t_tile[(blockIdx.x / (cols / 32U) * 128U +
-                        threadIdx.x / 2U * 8U + resIdxM) * cols +
-                       blockIdx.x % (cols / 32U) * 32U +
-                       threadIdx.x % 2U * 16U + resIdxN]
+                t_tile[(128U * (blockIdx.x / (cols / 32U)) +
+                        8U * (threadIdx.x / 2U) + resIdxM) * cols +
+                       32U * (blockIdx.x % (cols / 32U)) +
+                       16U * (threadIdx.x % 2U) + resIdxN]
                 + alpha * rchProd[resIdxM * 16U + resIdxN];
     }
 }
@@ -5427,6 +5527,7 @@ __hoisted_50(float alpha,
             for (; k < 4U; k++)
                 sA[(col + k) * 128U + row] = local[k];
         }
+        uint32_t __anf06 = bkIdx;
         float *tileB = gB;
         uint32_t i = 0U;
         for (; i < 1024U; i += 128U) {
@@ -5435,7 +5536,7 @@ __hoisted_50(float alpha,
             uint32_t row = (i + threadIdx.x * 4U) / 32U;
             uint32_t col = (i + threadIdx.x * 4U) % 32U;
             vec_memcpy(local,
-                       tileB + cols * (__anf03 * 32U) + mcol * 32U +
+                       tileB + cols * (__anf06 * 32U) + mcol * 32U +
                        cols * row + col);
             uint32_t k = 0U;
             for (; k < 4U; k++)
@@ -5469,14 +5570,15 @@ __hoisted_50(float alpha,
     for (; resIdxM < 16U; resIdxM++) {
         uint32_t resIdxN = 0U;
         for (; resIdxN < 8U; resIdxN++)
-            t_tile[(blockIdx.x / (cols / 32U) * 128U + threadIdx.x / 4U * 16U +
-                    resIdxM) * cols + blockIdx.x % (cols / 32U) * 32U +
-                   threadIdx.x % 4U * 8U + resIdxN]
+            t_tile[(128U * (blockIdx.x / (cols / 32U)) +
+                    16U * (threadIdx.x / 4U) + resIdxM) * cols +
+                   32U * (blockIdx.x % (cols / 32U)) + 8U * (threadIdx.x % 4U) +
+                   resIdxN]
                 = beta *
-                t_tile[(blockIdx.x / (cols / 32U) * 128U +
-                        threadIdx.x / 4U * 16U + resIdxM) * cols +
-                       blockIdx.x % (cols / 32U) * 32U + threadIdx.x % 4U * 8U +
-                       resIdxN]
+                t_tile[(128U * (blockIdx.x / (cols / 32U)) +
+                        16U * (threadIdx.x / 4U) + resIdxM) * cols +
+                       32U * (blockIdx.x % (cols / 32U)) +
+                       8U * (threadIdx.x % 4U) + resIdxN]
                 + alpha * rchProd[resIdxM * 8U + resIdxN];
     }
 }
@@ -5535,6 +5637,7 @@ __hoisted_51(float alpha,
             for (; k < 4U; k++)
                 sA[(col + k) * 128U + row] = local[k];
         }
+        uint32_t __anf06 = bkIdx;
         float *tileB = gB;
         uint32_t i = 0U;
         for (; i < 1024U; i += 64U) {
@@ -5543,7 +5646,7 @@ __hoisted_51(float alpha,
             uint32_t row = (i + threadIdx.x * 4U) / 32U;
             uint32_t col = (i + threadIdx.x * 4U) % 32U;
             vec_memcpy(local,
-                       tileB + cols * (__anf03 * 32U) + mcol * 32U +
+                       tileB + cols * (__anf06 * 32U) + mcol * 32U +
                        cols * row + col);
             uint32_t k = 0U;
             for (; k < 4U; k++)
@@ -5577,14 +5680,15 @@ __hoisted_51(float alpha,
     for (; resIdxM < 16U; resIdxM++) {
         uint32_t resIdxN = 0U;
         for (; resIdxN < 16U; resIdxN++)
-            t_tile[(blockIdx.x / (cols / 32U) * 128U + threadIdx.x / 2U * 16U +
-                    resIdxM) * cols + blockIdx.x % (cols / 32U) * 32U +
-                   threadIdx.x % 2U * 16U + resIdxN]
+            t_tile[(128U * (blockIdx.x / (cols / 32U)) +
+                    16U * (threadIdx.x / 2U) + resIdxM) * cols +
+                   32U * (blockIdx.x % (cols / 32U)) +
+                   16U * (threadIdx.x % 2U) + resIdxN]
                 = beta *
-                t_tile[(blockIdx.x / (cols / 32U) * 128U +
-                        threadIdx.x / 2U * 16U + resIdxM) * cols +
-                       blockIdx.x % (cols / 32U) * 32U +
-                       threadIdx.x % 2U * 16U + resIdxN]
+                t_tile[(128U * (blockIdx.x / (cols / 32U)) +
+                        16U * (threadIdx.x / 2U) + resIdxM) * cols +
+                       32U * (blockIdx.x % (cols / 32U)) +
+                       16U * (threadIdx.x % 2U) + resIdxN]
                 + alpha * rchProd[resIdxM * 16U + resIdxN];
     }
 }
@@ -5643,6 +5747,7 @@ __hoisted_52(float alpha,
             for (; k < 4U; k++)
                 sA[(col + k) * 128U + row] = local[k];
         }
+        uint32_t __anf06 = bkIdx;
         float *tileB = gB;
         uint32_t i = 0U;
         for (; i < 2048U; i += 256U) {
@@ -5651,7 +5756,7 @@ __hoisted_52(float alpha,
             uint32_t row = (i + threadIdx.x * 4U) / 32U;
             uint32_t col = (i + threadIdx.x * 4U) % 32U;
             vec_memcpy(local,
-                       tileB + cols * (__anf03 * 64U) + mcol * 32U +
+                       tileB + cols * (__anf06 * 64U) + mcol * 32U +
                        cols * row + col);
             uint32_t k = 0U;
             for (; k < 4U; k++)
@@ -5685,14 +5790,15 @@ __hoisted_52(float alpha,
     for (; resIdxM < 8U; resIdxM++) {
         uint32_t resIdxN = 0U;
         for (; resIdxN < 8U; resIdxN++)
-            t_tile[(blockIdx.x / (cols / 32U) * 128U + threadIdx.x / 4U * 8U +
-                    resIdxM) * cols + blockIdx.x % (cols / 32U) * 32U +
-                   threadIdx.x % 4U * 8U + resIdxN]
+            t_tile[(128U * (blockIdx.x / (cols / 32U)) +
+                    8U * (threadIdx.x / 4U) + resIdxM) * cols +
+                   32U * (blockIdx.x % (cols / 32U)) + 8U * (threadIdx.x % 4U) +
+                   resIdxN]
                 = beta *
-                t_tile[(blockIdx.x / (cols / 32U) * 128U +
-                        threadIdx.x / 4U * 8U + resIdxM) * cols +
-                       blockIdx.x % (cols / 32U) * 32U + threadIdx.x % 4U * 8U +
-                       resIdxN]
+                t_tile[(128U * (blockIdx.x / (cols / 32U)) +
+                        8U * (threadIdx.x / 4U) + resIdxM) * cols +
+                       32U * (blockIdx.x % (cols / 32U)) +
+                       8U * (threadIdx.x % 4U) + resIdxN]
                 + alpha * rchProd[resIdxM * 8U + resIdxN];
     }
 }
@@ -5751,6 +5857,7 @@ __hoisted_53(float alpha,
             for (; k < 4U; k++)
                 sA[(col + k) * 128U + row] = local[k];
         }
+        uint32_t __anf06 = bkIdx;
         float *tileB = gB;
         uint32_t i = 0U;
         for (; i < 2048U; i += 128U) {
@@ -5759,7 +5866,7 @@ __hoisted_53(float alpha,
             uint32_t row = (i + threadIdx.x * 4U) / 32U;
             uint32_t col = (i + threadIdx.x * 4U) % 32U;
             vec_memcpy(local,
-                       tileB + cols * (__anf03 * 64U) + mcol * 32U +
+                       tileB + cols * (__anf06 * 64U) + mcol * 32U +
                        cols * row + col);
             uint32_t k = 0U;
             for (; k < 4U; k++)
@@ -5793,14 +5900,15 @@ __hoisted_53(float alpha,
     for (; resIdxM < 8U; resIdxM++) {
         uint32_t resIdxN = 0U;
         for (; resIdxN < 16U; resIdxN++)
-            t_tile[(blockIdx.x / (cols / 32U) * 128U + threadIdx.x / 2U * 8U +
-                    resIdxM) * cols + blockIdx.x % (cols / 32U) * 32U +
-                   threadIdx.x % 2U * 16U + resIdxN]
+            t_tile[(128U * (blockIdx.x / (cols / 32U)) +
+                    8U * (threadIdx.x / 2U) + resIdxM) * cols +
+                   32U * (blockIdx.x % (cols / 32U)) +
+                   16U * (threadIdx.x % 2U) + resIdxN]
                 = beta *
-                t_tile[(blockIdx.x / (cols / 32U) * 128U +
-                        threadIdx.x / 2U * 8U + resIdxM) * cols +
-                       blockIdx.x % (cols / 32U) * 32U +
-                       threadIdx.x % 2U * 16U + resIdxN]
+                t_tile[(128U * (blockIdx.x / (cols / 32U)) +
+                        8U * (threadIdx.x / 2U) + resIdxM) * cols +
+                       32U * (blockIdx.x % (cols / 32U)) +
+                       16U * (threadIdx.x % 2U) + resIdxN]
                 + alpha * rchProd[resIdxM * 16U + resIdxN];
     }
 }
@@ -5859,6 +5967,7 @@ __hoisted_54(float alpha,
             for (; k < 4U; k++)
                 sA[(col + k) * 128U + row] = local[k];
         }
+        uint32_t __anf06 = bkIdx;
         float *tileB = gB;
         uint32_t i = 0U;
         for (; i < 2048U; i += 128U) {
@@ -5867,7 +5976,7 @@ __hoisted_54(float alpha,
             uint32_t row = (i + threadIdx.x * 4U) / 32U;
             uint32_t col = (i + threadIdx.x * 4U) % 32U;
             vec_memcpy(local,
-                       tileB + cols * (__anf03 * 64U) + mcol * 32U +
+                       tileB + cols * (__anf06 * 64U) + mcol * 32U +
                        cols * row + col);
             uint32_t k = 0U;
             for (; k < 4U; k++)
@@ -5901,14 +6010,15 @@ __hoisted_54(float alpha,
     for (; resIdxM < 16U; resIdxM++) {
         uint32_t resIdxN = 0U;
         for (; resIdxN < 8U; resIdxN++)
-            t_tile[(blockIdx.x / (cols / 32U) * 128U + threadIdx.x / 4U * 16U +
-                    resIdxM) * cols + blockIdx.x % (cols / 32U) * 32U +
-                   threadIdx.x % 4U * 8U + resIdxN]
+            t_tile[(128U * (blockIdx.x / (cols / 32U)) +
+                    16U * (threadIdx.x / 4U) + resIdxM) * cols +
+                   32U * (blockIdx.x % (cols / 32U)) + 8U * (threadIdx.x % 4U) +
+                   resIdxN]
                 = beta *
-                t_tile[(blockIdx.x / (cols / 32U) * 128U +
-                        threadIdx.x / 4U * 16U + resIdxM) * cols +
-                       blockIdx.x % (cols / 32U) * 32U + threadIdx.x % 4U * 8U +
-                       resIdxN]
+                t_tile[(128U * (blockIdx.x / (cols / 32U)) +
+                        16U * (threadIdx.x / 4U) + resIdxM) * cols +
+                       32U * (blockIdx.x % (cols / 32U)) +
+                       8U * (threadIdx.x % 4U) + resIdxN]
                 + alpha * rchProd[resIdxM * 8U + resIdxN];
     }
 }
@@ -5967,6 +6077,7 @@ __hoisted_55(float alpha,
             for (; k < 4U; k++)
                 sA[(col + k) * 128U + row] = local[k];
         }
+        uint32_t __anf06 = bkIdx;
         float *tileB = gB;
         uint32_t i = 0U;
         for (; i < 2048U; i += 64U) {
@@ -5975,7 +6086,7 @@ __hoisted_55(float alpha,
             uint32_t row = (i + threadIdx.x * 4U) / 32U;
             uint32_t col = (i + threadIdx.x * 4U) % 32U;
             vec_memcpy(local,
-                       tileB + cols * (__anf03 * 64U) + mcol * 32U +
+                       tileB + cols * (__anf06 * 64U) + mcol * 32U +
                        cols * row + col);
             uint32_t k = 0U;
             for (; k < 4U; k++)
@@ -6009,14 +6120,15 @@ __hoisted_55(float alpha,
     for (; resIdxM < 16U; resIdxM++) {
         uint32_t resIdxN = 0U;
         for (; resIdxN < 16U; resIdxN++)
-            t_tile[(blockIdx.x / (cols / 32U) * 128U + threadIdx.x / 2U * 16U +
-                    resIdxM) * cols + blockIdx.x % (cols / 32U) * 32U +
-                   threadIdx.x % 2U * 16U + resIdxN]
+            t_tile[(128U * (blockIdx.x / (cols / 32U)) +
+                    16U * (threadIdx.x / 2U) + resIdxM) * cols +
+                   32U * (blockIdx.x % (cols / 32U)) +
+                   16U * (threadIdx.x % 2U) + resIdxN]
                 = beta *
-                t_tile[(blockIdx.x / (cols / 32U) * 128U +
-                        threadIdx.x / 2U * 16U + resIdxM) * cols +
-                       blockIdx.x % (cols / 32U) * 32U +
-                       threadIdx.x % 2U * 16U + resIdxN]
+                t_tile[(128U * (blockIdx.x / (cols / 32U)) +
+                        16U * (threadIdx.x / 2U) + resIdxM) * cols +
+                       32U * (blockIdx.x % (cols / 32U)) +
+                       16U * (threadIdx.x % 2U) + resIdxN]
                 + alpha * rchProd[resIdxM * 16U + resIdxN];
     }
 }
@@ -6075,6 +6187,7 @@ __hoisted_56(float alpha,
             for (; k < 4U; k++)
                 sA[(col + k) * 128U + row] = local[k];
         }
+        uint32_t __anf06 = bkIdx;
         float *tileB = gB;
         uint32_t i = 0U;
         for (; i < 2048U; i += 512U) {
@@ -6083,7 +6196,7 @@ __hoisted_56(float alpha,
             uint32_t row = (i + threadIdx.x * 4U) / 64U;
             uint32_t col = (i + threadIdx.x * 4U) % 64U;
             vec_memcpy(local,
-                       tileB + cols * (__anf03 * 32U) + mcol * 64U +
+                       tileB + cols * (__anf06 * 32U) + mcol * 64U +
                        cols * row + col);
             uint32_t k = 0U;
             for (; k < 4U; k++)
@@ -6117,14 +6230,15 @@ __hoisted_56(float alpha,
     for (; resIdxM < 8U; resIdxM++) {
         uint32_t resIdxN = 0U;
         for (; resIdxN < 8U; resIdxN++)
-            t_tile[(blockIdx.x / (cols / 64U) * 128U + threadIdx.x / 8U * 8U +
-                    resIdxM) * cols + blockIdx.x % (cols / 64U) * 64U +
-                   threadIdx.x % 8U * 8U + resIdxN]
+            t_tile[(128U * (blockIdx.x / (cols / 64U)) +
+                    8U * (threadIdx.x / 8U) + resIdxM) * cols +
+                   64U * (blockIdx.x % (cols / 64U)) + 8U * (threadIdx.x % 8U) +
+                   resIdxN]
                 = beta *
-                t_tile[(blockIdx.x / (cols / 64U) * 128U +
-                        threadIdx.x / 8U * 8U + resIdxM) * cols +
-                       blockIdx.x % (cols / 64U) * 64U + threadIdx.x % 8U * 8U +
-                       resIdxN]
+                t_tile[(128U * (blockIdx.x / (cols / 64U)) +
+                        8U * (threadIdx.x / 8U) + resIdxM) * cols +
+                       64U * (blockIdx.x % (cols / 64U)) +
+                       8U * (threadIdx.x % 8U) + resIdxN]
                 + alpha * rchProd[resIdxM * 8U + resIdxN];
     }
 }
@@ -6183,6 +6297,7 @@ __hoisted_57(float alpha,
             for (; k < 4U; k++)
                 sA[(col + k) * 128U + row] = local[k];
         }
+        uint32_t __anf06 = bkIdx;
         float *tileB = gB;
         uint32_t i = 0U;
         for (; i < 2048U; i += 256U) {
@@ -6191,7 +6306,7 @@ __hoisted_57(float alpha,
             uint32_t row = (i + threadIdx.x * 4U) / 64U;
             uint32_t col = (i + threadIdx.x * 4U) % 64U;
             vec_memcpy(local,
-                       tileB + cols * (__anf03 * 32U) + mcol * 64U +
+                       tileB + cols * (__anf06 * 32U) + mcol * 64U +
                        cols * row + col);
             uint32_t k = 0U;
             for (; k < 4U; k++)
@@ -6225,14 +6340,15 @@ __hoisted_57(float alpha,
     for (; resIdxM < 8U; resIdxM++) {
         uint32_t resIdxN = 0U;
         for (; resIdxN < 16U; resIdxN++)
-            t_tile[(blockIdx.x / (cols / 64U) * 128U + threadIdx.x / 4U * 8U +
-                    resIdxM) * cols + blockIdx.x % (cols / 64U) * 64U +
-                   threadIdx.x % 4U * 16U + resIdxN]
+            t_tile[(128U * (blockIdx.x / (cols / 64U)) +
+                    8U * (threadIdx.x / 4U) + resIdxM) * cols +
+                   64U * (blockIdx.x % (cols / 64U)) +
+                   16U * (threadIdx.x % 4U) + resIdxN]
                 = beta *
-                t_tile[(blockIdx.x / (cols / 64U) * 128U +
-                        threadIdx.x / 4U * 8U + resIdxM) * cols +
-                       blockIdx.x % (cols / 64U) * 64U +
-                       threadIdx.x % 4U * 16U + resIdxN]
+                t_tile[(128U * (blockIdx.x / (cols / 64U)) +
+                        8U * (threadIdx.x / 4U) + resIdxM) * cols +
+                       64U * (blockIdx.x % (cols / 64U)) +
+                       16U * (threadIdx.x % 4U) + resIdxN]
                 + alpha * rchProd[resIdxM * 16U + resIdxN];
     }
 }
@@ -6291,6 +6407,7 @@ __hoisted_58(float alpha,
             for (; k < 4U; k++)
                 sA[(col + k) * 128U + row] = local[k];
         }
+        uint32_t __anf06 = bkIdx;
         float *tileB = gB;
         uint32_t i = 0U;
         for (; i < 2048U; i += 256U) {
@@ -6299,7 +6416,7 @@ __hoisted_58(float alpha,
             uint32_t row = (i + threadIdx.x * 4U) / 64U;
             uint32_t col = (i + threadIdx.x * 4U) % 64U;
             vec_memcpy(local,
-                       tileB + cols * (__anf03 * 32U) + mcol * 64U +
+                       tileB + cols * (__anf06 * 32U) + mcol * 64U +
                        cols * row + col);
             uint32_t k = 0U;
             for (; k < 4U; k++)
@@ -6333,14 +6450,15 @@ __hoisted_58(float alpha,
     for (; resIdxM < 16U; resIdxM++) {
         uint32_t resIdxN = 0U;
         for (; resIdxN < 8U; resIdxN++)
-            t_tile[(blockIdx.x / (cols / 64U) * 128U + threadIdx.x / 8U * 16U +
-                    resIdxM) * cols + blockIdx.x % (cols / 64U) * 64U +
-                   threadIdx.x % 8U * 8U + resIdxN]
+            t_tile[(128U * (blockIdx.x / (cols / 64U)) +
+                    16U * (threadIdx.x / 8U) + resIdxM) * cols +
+                   64U * (blockIdx.x % (cols / 64U)) + 8U * (threadIdx.x % 8U) +
+                   resIdxN]
                 = beta *
-                t_tile[(blockIdx.x / (cols / 64U) * 128U +
-                        threadIdx.x / 8U * 16U + resIdxM) * cols +
-                       blockIdx.x % (cols / 64U) * 64U + threadIdx.x % 8U * 8U +
-                       resIdxN]
+                t_tile[(128U * (blockIdx.x / (cols / 64U)) +
+                        16U * (threadIdx.x / 8U) + resIdxM) * cols +
+                       64U * (blockIdx.x % (cols / 64U)) +
+                       8U * (threadIdx.x % 8U) + resIdxN]
                 + alpha * rchProd[resIdxM * 8U + resIdxN];
     }
 }
@@ -6399,6 +6517,7 @@ __hoisted_59(float alpha,
             for (; k < 4U; k++)
                 sA[(col + k) * 128U + row] = local[k];
         }
+        uint32_t __anf06 = bkIdx;
         float *tileB = gB;
         uint32_t i = 0U;
         for (; i < 2048U; i += 128U) {
@@ -6407,7 +6526,7 @@ __hoisted_59(float alpha,
             uint32_t row = (i + threadIdx.x * 4U) / 64U;
             uint32_t col = (i + threadIdx.x * 4U) % 64U;
             vec_memcpy(local,
-                       tileB + cols * (__anf03 * 32U) + mcol * 64U +
+                       tileB + cols * (__anf06 * 32U) + mcol * 64U +
                        cols * row + col);
             uint32_t k = 0U;
             for (; k < 4U; k++)
@@ -6441,14 +6560,15 @@ __hoisted_59(float alpha,
     for (; resIdxM < 16U; resIdxM++) {
         uint32_t resIdxN = 0U;
         for (; resIdxN < 16U; resIdxN++)
-            t_tile[(blockIdx.x / (cols / 64U) * 128U + threadIdx.x / 4U * 16U +
-                    resIdxM) * cols + blockIdx.x % (cols / 64U) * 64U +
-                   threadIdx.x % 4U * 16U + resIdxN]
+            t_tile[(128U * (blockIdx.x / (cols / 64U)) +
+                    16U * (threadIdx.x / 4U) + resIdxM) * cols +
+                   64U * (blockIdx.x % (cols / 64U)) +
+                   16U * (threadIdx.x % 4U) + resIdxN]
                 = beta *
-                t_tile[(blockIdx.x / (cols / 64U) * 128U +
-                        threadIdx.x / 4U * 16U + resIdxM) * cols +
-                       blockIdx.x % (cols / 64U) * 64U +
-                       threadIdx.x % 4U * 16U + resIdxN]
+                t_tile[(128U * (blockIdx.x / (cols / 64U)) +
+                        16U * (threadIdx.x / 4U) + resIdxM) * cols +
+                       64U * (blockIdx.x % (cols / 64U)) +
+                       16U * (threadIdx.x % 4U) + resIdxN]
                 + alpha * rchProd[resIdxM * 16U + resIdxN];
     }
 }
@@ -6507,6 +6627,7 @@ __hoisted_60(float alpha,
             for (; k < 4U; k++)
                 sA[(col + k) * 128U + row] = local[k];
         }
+        uint32_t __anf06 = bkIdx;
         float *tileB = gB;
         uint32_t i = 0U;
         for (; i < 4096U; i += 512U) {
@@ -6515,7 +6636,7 @@ __hoisted_60(float alpha,
             uint32_t row = (i + threadIdx.x * 4U) / 64U;
             uint32_t col = (i + threadIdx.x * 4U) % 64U;
             vec_memcpy(local,
-                       tileB + cols * (__anf03 * 64U) + mcol * 64U +
+                       tileB + cols * (__anf06 * 64U) + mcol * 64U +
                        cols * row + col);
             uint32_t k = 0U;
             for (; k < 4U; k++)
@@ -6549,14 +6670,15 @@ __hoisted_60(float alpha,
     for (; resIdxM < 8U; resIdxM++) {
         uint32_t resIdxN = 0U;
         for (; resIdxN < 8U; resIdxN++)
-            t_tile[(blockIdx.x / (cols / 64U) * 128U + threadIdx.x / 8U * 8U +
-                    resIdxM) * cols + blockIdx.x % (cols / 64U) * 64U +
-                   threadIdx.x % 8U * 8U + resIdxN]
+            t_tile[(128U * (blockIdx.x / (cols / 64U)) +
+                    8U * (threadIdx.x / 8U) + resIdxM) * cols +
+                   64U * (blockIdx.x % (cols / 64U)) + 8U * (threadIdx.x % 8U) +
+                   resIdxN]
                 = beta *
-                t_tile[(blockIdx.x / (cols / 64U) * 128U +
-                        threadIdx.x / 8U * 8U + resIdxM) * cols +
-                       blockIdx.x % (cols / 64U) * 64U + threadIdx.x % 8U * 8U +
-                       resIdxN]
+                t_tile[(128U * (blockIdx.x / (cols / 64U)) +
+                        8U * (threadIdx.x / 8U) + resIdxM) * cols +
+                       64U * (blockIdx.x % (cols / 64U)) +
+                       8U * (threadIdx.x % 8U) + resIdxN]
                 + alpha * rchProd[resIdxM * 8U + resIdxN];
     }
 }
@@ -6615,6 +6737,7 @@ __hoisted_61(float alpha,
             for (; k < 4U; k++)
                 sA[(col + k) * 128U + row] = local[k];
         }
+        uint32_t __anf06 = bkIdx;
         float *tileB = gB;
         uint32_t i = 0U;
         for (; i < 4096U; i += 256U) {
@@ -6623,7 +6746,7 @@ __hoisted_61(float alpha,
             uint32_t row = (i + threadIdx.x * 4U) / 64U;
             uint32_t col = (i + threadIdx.x * 4U) % 64U;
             vec_memcpy(local,
-                       tileB + cols * (__anf03 * 64U) + mcol * 64U +
+                       tileB + cols * (__anf06 * 64U) + mcol * 64U +
                        cols * row + col);
             uint32_t k = 0U;
             for (; k < 4U; k++)
@@ -6657,14 +6780,15 @@ __hoisted_61(float alpha,
     for (; resIdxM < 8U; resIdxM++) {
         uint32_t resIdxN = 0U;
         for (; resIdxN < 16U; resIdxN++)
-            t_tile[(blockIdx.x / (cols / 64U) * 128U + threadIdx.x / 4U * 8U +
-                    resIdxM) * cols + blockIdx.x % (cols / 64U) * 64U +
-                   threadIdx.x % 4U * 16U + resIdxN]
+            t_tile[(128U * (blockIdx.x / (cols / 64U)) +
+                    8U * (threadIdx.x / 4U) + resIdxM) * cols +
+                   64U * (blockIdx.x % (cols / 64U)) +
+                   16U * (threadIdx.x % 4U) + resIdxN]
                 = beta *
-                t_tile[(blockIdx.x / (cols / 64U) * 128U +
-                        threadIdx.x / 4U * 8U + resIdxM) * cols +
-                       blockIdx.x % (cols / 64U) * 64U +
-                       threadIdx.x % 4U * 16U + resIdxN]
+                t_tile[(128U * (blockIdx.x / (cols / 64U)) +
+                        8U * (threadIdx.x / 4U) + resIdxM) * cols +
+                       64U * (blockIdx.x % (cols / 64U)) +
+                       16U * (threadIdx.x % 4U) + resIdxN]
                 + alpha * rchProd[resIdxM * 16U + resIdxN];
     }
 }
@@ -6723,6 +6847,7 @@ __hoisted_62(float alpha,
             for (; k < 4U; k++)
                 sA[(col + k) * 128U + row] = local[k];
         }
+        uint32_t __anf06 = bkIdx;
         float *tileB = gB;
         uint32_t i = 0U;
         for (; i < 4096U; i += 256U) {
@@ -6731,7 +6856,7 @@ __hoisted_62(float alpha,
             uint32_t row = (i + threadIdx.x * 4U) / 64U;
             uint32_t col = (i + threadIdx.x * 4U) % 64U;
             vec_memcpy(local,
-                       tileB + cols * (__anf03 * 64U) + mcol * 64U +
+                       tileB + cols * (__anf06 * 64U) + mcol * 64U +
                        cols * row + col);
             uint32_t k = 0U;
             for (; k < 4U; k++)
@@ -6765,14 +6890,15 @@ __hoisted_62(float alpha,
     for (; resIdxM < 16U; resIdxM++) {
         uint32_t resIdxN = 0U;
         for (; resIdxN < 8U; resIdxN++)
-            t_tile[(blockIdx.x / (cols / 64U) * 128U + threadIdx.x / 8U * 16U +
-                    resIdxM) * cols + blockIdx.x % (cols / 64U) * 64U +
-                   threadIdx.x % 8U * 8U + resIdxN]
+            t_tile[(128U * (blockIdx.x / (cols / 64U)) +
+                    16U * (threadIdx.x / 8U) + resIdxM) * cols +
+                   64U * (blockIdx.x % (cols / 64U)) + 8U * (threadIdx.x % 8U) +
+                   resIdxN]
                 = beta *
-                t_tile[(blockIdx.x / (cols / 64U) * 128U +
-                        threadIdx.x / 8U * 16U + resIdxM) * cols +
-                       blockIdx.x % (cols / 64U) * 64U + threadIdx.x % 8U * 8U +
-                       resIdxN]
+                t_tile[(128U * (blockIdx.x / (cols / 64U)) +
+                        16U * (threadIdx.x / 8U) + resIdxM) * cols +
+                       64U * (blockIdx.x % (cols / 64U)) +
+                       8U * (threadIdx.x % 8U) + resIdxN]
                 + alpha * rchProd[resIdxM * 8U + resIdxN];
     }
 }
@@ -6831,6 +6957,7 @@ __hoisted_63(float alpha,
             for (; k < 4U; k++)
                 sA[(col + k) * 128U + row] = local[k];
         }
+        uint32_t __anf06 = bkIdx;
         float *tileB = gB;
         uint32_t i = 0U;
         for (; i < 4096U; i += 128U) {
@@ -6839,7 +6966,7 @@ __hoisted_63(float alpha,
             uint32_t row = (i + threadIdx.x * 4U) / 64U;
             uint32_t col = (i + threadIdx.x * 4U) % 64U;
             vec_memcpy(local,
-                       tileB + cols * (__anf03 * 64U) + mcol * 64U +
+                       tileB + cols * (__anf06 * 64U) + mcol * 64U +
                        cols * row + col);
             uint32_t k = 0U;
             for (; k < 4U; k++)
@@ -6873,14 +7000,15 @@ __hoisted_63(float alpha,
     for (; resIdxM < 16U; resIdxM++) {
         uint32_t resIdxN = 0U;
         for (; resIdxN < 16U; resIdxN++)
-            t_tile[(blockIdx.x / (cols / 64U) * 128U + threadIdx.x / 4U * 16U +
-                    resIdxM) * cols + blockIdx.x % (cols / 64U) * 64U +
-                   threadIdx.x % 4U * 16U + resIdxN]
+            t_tile[(128U * (blockIdx.x / (cols / 64U)) +
+                    16U * (threadIdx.x / 4U) + resIdxM) * cols +
+                   64U * (blockIdx.x % (cols / 64U)) +
+                   16U * (threadIdx.x % 4U) + resIdxN]
                 = beta *
-                t_tile[(blockIdx.x / (cols / 64U) * 128U +
-                        threadIdx.x / 4U * 16U + resIdxM) * cols +
-                       blockIdx.x % (cols / 64U) * 64U +
-                       threadIdx.x % 4U * 16U + resIdxN]
+                t_tile[(128U * (blockIdx.x / (cols / 64U)) +
+                        16U * (threadIdx.x / 4U) + resIdxM) * cols +
+                       64U * (blockIdx.x % (cols / 64U)) +
+                       16U * (threadIdx.x % 4U) + resIdxN]
                 + alpha * rchProd[resIdxM * 16U + resIdxN];
     }
 }
@@ -6939,6 +7067,7 @@ __hoisted_64(float alpha,
             for (; k < 4U; k++)
                 sA[(col + k) * 128U + row] = local[k];
         }
+        uint32_t __anf06 = bkIdx;
         float *tileB = gB;
         uint32_t i = 0U;
         for (; i < 4096U; i += 1024U) {
@@ -6947,7 +7076,7 @@ __hoisted_64(float alpha,
             uint32_t row = (i + threadIdx.x * 4U) / 128U;
             uint32_t col = (i + threadIdx.x * 4U) % 128U;
             vec_memcpy(local,
-                       tileB + cols * (__anf03 * 32U) + mcol * 128U +
+                       tileB + cols * (__anf06 * 32U) + mcol * 128U +
                        cols * row + col);
             uint32_t k = 0U;
             for (; k < 4U; k++)
@@ -6981,14 +7110,15 @@ __hoisted_64(float alpha,
     for (; resIdxM < 8U; resIdxM++) {
         uint32_t resIdxN = 0U;
         for (; resIdxN < 8U; resIdxN++)
-            t_tile[(blockIdx.x / (cols / 128U) * 128U + threadIdx.x / 16U * 8U +
-                    resIdxM) * cols + blockIdx.x % (cols / 128U) * 128U +
-                   threadIdx.x % 16U * 8U + resIdxN]
+            t_tile[(128U * (blockIdx.x / (cols / 128U)) +
+                    8U * (threadIdx.x / 16U) + resIdxM) * cols +
+                   128U * (blockIdx.x % (cols / 128U)) +
+                   8U * (threadIdx.x % 16U) + resIdxN]
                 = beta *
-                t_tile[(blockIdx.x / (cols / 128U) * 128U +
-                        threadIdx.x / 16U * 8U + resIdxM) * cols +
-                       blockIdx.x % (cols / 128U) * 128U +
-                       threadIdx.x % 16U * 8U + resIdxN]
+                t_tile[(128U * (blockIdx.x / (cols / 128U)) +
+                        8U * (threadIdx.x / 16U) + resIdxM) * cols +
+                       128U * (blockIdx.x % (cols / 128U)) +
+                       8U * (threadIdx.x % 16U) + resIdxN]
                 + alpha * rchProd[resIdxM * 8U + resIdxN];
     }
 }
@@ -7047,6 +7177,7 @@ __hoisted_65(float alpha,
             for (; k < 4U; k++)
                 sA[(col + k) * 128U + row] = local[k];
         }
+        uint32_t __anf06 = bkIdx;
         float *tileB = gB;
         uint32_t i = 0U;
         for (; i < 4096U; i += 512U) {
@@ -7055,7 +7186,7 @@ __hoisted_65(float alpha,
             uint32_t row = (i + threadIdx.x * 4U) / 128U;
             uint32_t col = (i + threadIdx.x * 4U) % 128U;
             vec_memcpy(local,
-                       tileB + cols * (__anf03 * 32U) + mcol * 128U +
+                       tileB + cols * (__anf06 * 32U) + mcol * 128U +
                        cols * row + col);
             uint32_t k = 0U;
             for (; k < 4U; k++)
@@ -7089,14 +7220,15 @@ __hoisted_65(float alpha,
     for (; resIdxM < 8U; resIdxM++) {
         uint32_t resIdxN = 0U;
         for (; resIdxN < 16U; resIdxN++)
-            t_tile[(blockIdx.x / (cols / 128U) * 128U + threadIdx.x / 8U * 8U +
-                    resIdxM) * cols + blockIdx.x % (cols / 128U) * 128U +
-                   threadIdx.x % 8U * 16U + resIdxN]
+            t_tile[(128U * (blockIdx.x / (cols / 128U)) +
+                    8U * (threadIdx.x / 8U) + resIdxM) * cols +
+                   128U * (blockIdx.x % (cols / 128U)) +
+                   16U * (threadIdx.x % 8U) + resIdxN]
                 = beta *
-                t_tile[(blockIdx.x / (cols / 128U) * 128U +
-                        threadIdx.x / 8U * 8U + resIdxM) * cols +
-                       blockIdx.x % (cols / 128U) * 128U +
-                       threadIdx.x % 8U * 16U + resIdxN]
+                t_tile[(128U * (blockIdx.x / (cols / 128U)) +
+                        8U * (threadIdx.x / 8U) + resIdxM) * cols +
+                       128U * (blockIdx.x % (cols / 128U)) +
+                       16U * (threadIdx.x % 8U) + resIdxN]
                 + alpha * rchProd[resIdxM * 16U + resIdxN];
     }
 }
@@ -7155,6 +7287,7 @@ __hoisted_66(float alpha,
             for (; k < 4U; k++)
                 sA[(col + k) * 128U + row] = local[k];
         }
+        uint32_t __anf06 = bkIdx;
         float *tileB = gB;
         uint32_t i = 0U;
         for (; i < 4096U; i += 512U) {
@@ -7163,7 +7296,7 @@ __hoisted_66(float alpha,
             uint32_t row = (i + threadIdx.x * 4U) / 128U;
             uint32_t col = (i + threadIdx.x * 4U) % 128U;
             vec_memcpy(local,
-                       tileB + cols * (__anf03 * 32U) + mcol * 128U +
+                       tileB + cols * (__anf06 * 32U) + mcol * 128U +
                        cols * row + col);
             uint32_t k = 0U;
             for (; k < 4U; k++)
@@ -7197,15 +7330,15 @@ __hoisted_66(float alpha,
     for (; resIdxM < 16U; resIdxM++) {
         uint32_t resIdxN = 0U;
         for (; resIdxN < 8U; resIdxN++)
-            t_tile[(blockIdx.x / (cols / 128U) * 128U +
-                    threadIdx.x / 16U * 16U + resIdxM) * cols +
-                   blockIdx.x % (cols / 128U) * 128U + threadIdx.x % 16U * 8U +
-                   resIdxN]
+            t_tile[(128U * (blockIdx.x / (cols / 128U)) +
+                    16U * (threadIdx.x / 16U) + resIdxM) * cols +
+                   128U * (blockIdx.x % (cols / 128U)) +
+                   8U * (threadIdx.x % 16U) + resIdxN]
                 = beta *
-                t_tile[(blockIdx.x / (cols / 128U) * 128U +
-                        threadIdx.x / 16U * 16U + resIdxM) * cols +
-                       blockIdx.x % (cols / 128U) * 128U +
-                       threadIdx.x % 16U * 8U + resIdxN]
+                t_tile[(128U * (blockIdx.x / (cols / 128U)) +
+                        16U * (threadIdx.x / 16U) + resIdxM) * cols +
+                       128U * (blockIdx.x % (cols / 128U)) +
+                       8U * (threadIdx.x % 16U) + resIdxN]
                 + alpha * rchProd[resIdxM * 8U + resIdxN];
     }
 }
@@ -7264,6 +7397,7 @@ __hoisted_67(float alpha,
             for (; k < 4U; k++)
                 sA[(col + k) * 128U + row] = local[k];
         }
+        uint32_t __anf06 = bkIdx;
         float *tileB = gB;
         uint32_t i = 0U;
         for (; i < 4096U; i += 256U) {
@@ -7272,7 +7406,7 @@ __hoisted_67(float alpha,
             uint32_t row = (i + threadIdx.x * 4U) / 128U;
             uint32_t col = (i + threadIdx.x * 4U) % 128U;
             vec_memcpy(local,
-                       tileB + cols * (__anf03 * 32U) + mcol * 128U +
+                       tileB + cols * (__anf06 * 32U) + mcol * 128U +
                        cols * row + col);
             uint32_t k = 0U;
             for (; k < 4U; k++)
@@ -7306,14 +7440,15 @@ __hoisted_67(float alpha,
     for (; resIdxM < 16U; resIdxM++) {
         uint32_t resIdxN = 0U;
         for (; resIdxN < 16U; resIdxN++)
-            t_tile[(blockIdx.x / (cols / 128U) * 128U + threadIdx.x / 8U * 16U +
-                    resIdxM) * cols + blockIdx.x % (cols / 128U) * 128U +
-                   threadIdx.x % 8U * 16U + resIdxN]
+            t_tile[(128U * (blockIdx.x / (cols / 128U)) +
+                    16U * (threadIdx.x / 8U) + resIdxM) * cols +
+                   128U * (blockIdx.x % (cols / 128U)) +
+                   16U * (threadIdx.x % 8U) + resIdxN]
                 = beta *
-                t_tile[(blockIdx.x / (cols / 128U) * 128U +
-                        threadIdx.x / 8U * 16U + resIdxM) * cols +
-                       blockIdx.x % (cols / 128U) * 128U +
-                       threadIdx.x % 8U * 16U + resIdxN]
+                t_tile[(128U * (blockIdx.x / (cols / 128U)) +
+                        16U * (threadIdx.x / 8U) + resIdxM) * cols +
+                       128U * (blockIdx.x % (cols / 128U)) +
+                       16U * (threadIdx.x % 8U) + resIdxN]
                 + alpha * rchProd[resIdxM * 16U + resIdxN];
     }
 }
@@ -7372,6 +7507,7 @@ __hoisted_68(float alpha,
             for (; k < 4U; k++)
                 sA[(col + k) * 128U + row] = local[k];
         }
+        uint32_t __anf06 = bkIdx;
         float *tileB = gB;
         uint32_t i = 0U;
         for (; i < 8192U; i += 1024U) {
@@ -7380,7 +7516,7 @@ __hoisted_68(float alpha,
             uint32_t row = (i + threadIdx.x * 4U) / 128U;
             uint32_t col = (i + threadIdx.x * 4U) % 128U;
             vec_memcpy(local,
-                       tileB + cols * (__anf03 * 64U) + mcol * 128U +
+                       tileB + cols * (__anf06 * 64U) + mcol * 128U +
                        cols * row + col);
             uint32_t k = 0U;
             for (; k < 4U; k++)
@@ -7414,14 +7550,15 @@ __hoisted_68(float alpha,
     for (; resIdxM < 8U; resIdxM++) {
         uint32_t resIdxN = 0U;
         for (; resIdxN < 8U; resIdxN++)
-            t_tile[(blockIdx.x / (cols / 128U) * 128U + threadIdx.x / 16U * 8U +
-                    resIdxM) * cols + blockIdx.x % (cols / 128U) * 128U +
-                   threadIdx.x % 16U * 8U + resIdxN]
+            t_tile[(128U * (blockIdx.x / (cols / 128U)) +
+                    8U * (threadIdx.x / 16U) + resIdxM) * cols +
+                   128U * (blockIdx.x % (cols / 128U)) +
+                   8U * (threadIdx.x % 16U) + resIdxN]
                 = beta *
-                t_tile[(blockIdx.x / (cols / 128U) * 128U +
-                        threadIdx.x / 16U * 8U + resIdxM) * cols +
-                       blockIdx.x % (cols / 128U) * 128U +
-                       threadIdx.x % 16U * 8U + resIdxN]
+                t_tile[(128U * (blockIdx.x / (cols / 128U)) +
+                        8U * (threadIdx.x / 16U) + resIdxM) * cols +
+                       128U * (blockIdx.x % (cols / 128U)) +
+                       8U * (threadIdx.x % 16U) + resIdxN]
                 + alpha * rchProd[resIdxM * 8U + resIdxN];
     }
 }
@@ -7480,6 +7617,7 @@ __hoisted_69(float alpha,
             for (; k < 4U; k++)
                 sA[(col + k) * 128U + row] = local[k];
         }
+        uint32_t __anf06 = bkIdx;
         float *tileB = gB;
         uint32_t i = 0U;
         for (; i < 8192U; i += 512U) {
@@ -7488,7 +7626,7 @@ __hoisted_69(float alpha,
             uint32_t row = (i + threadIdx.x * 4U) / 128U;
             uint32_t col = (i + threadIdx.x * 4U) % 128U;
             vec_memcpy(local,
-                       tileB + cols * (__anf03 * 64U) + mcol * 128U +
+                       tileB + cols * (__anf06 * 64U) + mcol * 128U +
                        cols * row + col);
             uint32_t k = 0U;
             for (; k < 4U; k++)
@@ -7522,14 +7660,15 @@ __hoisted_69(float alpha,
     for (; resIdxM < 8U; resIdxM++) {
         uint32_t resIdxN = 0U;
         for (; resIdxN < 16U; resIdxN++)
-            t_tile[(blockIdx.x / (cols / 128U) * 128U + threadIdx.x / 8U * 8U +
-                    resIdxM) * cols + blockIdx.x % (cols / 128U) * 128U +
-                   threadIdx.x % 8U * 16U + resIdxN]
+            t_tile[(128U * (blockIdx.x / (cols / 128U)) +
+                    8U * (threadIdx.x / 8U) + resIdxM) * cols +
+                   128U * (blockIdx.x % (cols / 128U)) +
+                   16U * (threadIdx.x % 8U) + resIdxN]
                 = beta *
-                t_tile[(blockIdx.x / (cols / 128U) * 128U +
-                        threadIdx.x / 8U * 8U + resIdxM) * cols +
-                       blockIdx.x % (cols / 128U) * 128U +
-                       threadIdx.x % 8U * 16U + resIdxN]
+                t_tile[(128U * (blockIdx.x / (cols / 128U)) +
+                        8U * (threadIdx.x / 8U) + resIdxM) * cols +
+                       128U * (blockIdx.x % (cols / 128U)) +
+                       16U * (threadIdx.x % 8U) + resIdxN]
                 + alpha * rchProd[resIdxM * 16U + resIdxN];
     }
 }
@@ -7588,6 +7727,7 @@ __hoisted_70(float alpha,
             for (; k < 4U; k++)
                 sA[(col + k) * 128U + row] = local[k];
         }
+        uint32_t __anf06 = bkIdx;
         float *tileB = gB;
         uint32_t i = 0U;
         for (; i < 8192U; i += 512U) {
@@ -7596,7 +7736,7 @@ __hoisted_70(float alpha,
             uint32_t row = (i + threadIdx.x * 4U) / 128U;
             uint32_t col = (i + threadIdx.x * 4U) % 128U;
             vec_memcpy(local,
-                       tileB + cols * (__anf03 * 64U) + mcol * 128U +
+                       tileB + cols * (__anf06 * 64U) + mcol * 128U +
                        cols * row + col);
             uint32_t k = 0U;
             for (; k < 4U; k++)
@@ -7630,15 +7770,15 @@ __hoisted_70(float alpha,
     for (; resIdxM < 16U; resIdxM++) {
         uint32_t resIdxN = 0U;
         for (; resIdxN < 8U; resIdxN++)
-            t_tile[(blockIdx.x / (cols / 128U) * 128U +
-                    threadIdx.x / 16U * 16U + resIdxM) * cols +
-                   blockIdx.x % (cols / 128U) * 128U + threadIdx.x % 16U * 8U +
-                   resIdxN]
+            t_tile[(128U * (blockIdx.x / (cols / 128U)) +
+                    16U * (threadIdx.x / 16U) + resIdxM) * cols +
+                   128U * (blockIdx.x % (cols / 128U)) +
+                   8U * (threadIdx.x % 16U) + resIdxN]
                 = beta *
-                t_tile[(blockIdx.x / (cols / 128U) * 128U +
-                        threadIdx.x / 16U * 16U + resIdxM) * cols +
-                       blockIdx.x % (cols / 128U) * 128U +
-                       threadIdx.x % 16U * 8U + resIdxN]
+                t_tile[(128U * (blockIdx.x / (cols / 128U)) +
+                        16U * (threadIdx.x / 16U) + resIdxM) * cols +
+                       128U * (blockIdx.x % (cols / 128U)) +
+                       8U * (threadIdx.x % 16U) + resIdxN]
                 + alpha * rchProd[resIdxM * 8U + resIdxN];
     }
 }
@@ -7697,6 +7837,7 @@ __hoisted_71(float alpha,
             for (; k < 4U; k++)
                 sA[(col + k) * 128U + row] = local[k];
         }
+        uint32_t __anf06 = bkIdx;
         float *tileB = gB;
         uint32_t i = 0U;
         for (; i < 8192U; i += 256U) {
@@ -7705,7 +7846,7 @@ __hoisted_71(float alpha,
             uint32_t row = (i + threadIdx.x * 4U) / 128U;
             uint32_t col = (i + threadIdx.x * 4U) % 128U;
             vec_memcpy(local,
-                       tileB + cols * (__anf03 * 64U) + mcol * 128U +
+                       tileB + cols * (__anf06 * 64U) + mcol * 128U +
                        cols * row + col);
             uint32_t k = 0U;
             for (; k < 4U; k++)
@@ -7739,14 +7880,15 @@ __hoisted_71(float alpha,
     for (; resIdxM < 16U; resIdxM++) {
         uint32_t resIdxN = 0U;
         for (; resIdxN < 16U; resIdxN++)
-            t_tile[(blockIdx.x / (cols / 128U) * 128U + threadIdx.x / 8U * 16U +
-                    resIdxM) * cols + blockIdx.x % (cols / 128U) * 128U +
-                   threadIdx.x % 8U * 16U + resIdxN]
+            t_tile[(128U * (blockIdx.x / (cols / 128U)) +
+                    16U * (threadIdx.x / 8U) + resIdxM) * cols +
+                   128U * (blockIdx.x % (cols / 128U)) +
+                   16U * (threadIdx.x % 8U) + resIdxN]
                 = beta *
-                t_tile[(blockIdx.x / (cols / 128U) * 128U +
-                        threadIdx.x / 8U * 16U + resIdxM) * cols +
-                       blockIdx.x % (cols / 128U) * 128U +
-                       threadIdx.x % 8U * 16U + resIdxN]
+                t_tile[(128U * (blockIdx.x / (cols / 128U)) +
+                        16U * (threadIdx.x / 8U) + resIdxM) * cols +
+                       128U * (blockIdx.x % (cols / 128U)) +
+                       16U * (threadIdx.x % 8U) + resIdxN]
                 + alpha * rchProd[resIdxM * 16U + resIdxN];
     }
 }
